Multiple variables

transaction_kohler.v
@@ -19,6 +19,7 @@ Definition variable := nat.
 Definition store := NatMap.t value.
 Definition heap := address -> option (value * lock * version).
 Definition tid := nat.
+Definition addr := nat.
 
 
 Ltac myauto :=
@@ -31,22 +32,18 @@ end.
 
 
 Inductive action:=
-|start_txn: action
-|read_item: version -> action
-|write_item: value -> action
-|try_commit_txn: action
-|lock_write_item: action
-|seq_point: action
-|validate_read_item: version -> action
-|abort_txn: action
-|unlock_write_item: action
-(*|restart_txn: action*)
-|commit_txn: action
-|complete_write_item: (*value -> action*)version -> action
-(*|unlock_write_item: version -> action*)
-(*|invalid_write_item: value -> action*)
-|commit_done_txn: action.
-(*|obtain_global_tid: action.*)
+| start_txn : action
+| read_item : forall (ad:addr) (vers:version), action
+| write_item : forall (ad:addr) (val:value), action
+| try_commit_txn : action
+| lock_write_item : forall (ad:addr), action
+| seq_point : action
+| validate_read_item : forall (ad:addr) (vers:version), action
+| abort_txn : action
+| unlock_write_item : forall (ad:addr), action
+| commit_txn : action
+| complete_write_item : forall (ad:addr) (vers:version), action
+| commit_done_txn : action.
 (*sp later than last lock, but must before the first commit*)
 
 Lemma action_dec (a b:action):
@@ -63,17 +60,17 @@ Definition trace := list (tid * action).
 Definition action_phase (a:action) :=
   match a with
   | start_txn => 1
-  | read_item _ => 1
-  | write_item _ => 1
+  | read_item _ _ => 1
+  | write_item _ _ => 1
   | try_commit_txn => 2
-  | lock_write_item => 2
+  | lock_write_item _ => 2
   | seq_point => 3
-  | validate_read_item _ => 3
+  | validate_read_item _ _ => 3
   | commit_txn => 4
-  | complete_write_item _ => 4
+  | complete_write_item _ _ => 4
   | commit_done_txn => 4
   | abort_txn => 6
-  | unlock_write_item => 6
+  | unlock_write_item _ => 6
   end.
 
 Fixpoint tid_phase tid t: nat :=
@@ -178,32 +175,38 @@ Qed.
 
 
 (* Return the version number of the last committed write *)
-Fixpoint write_version (t:trace): version :=
+Fixpoint write_version (a:addr) (t:trace): version :=
   match t with
-  | (_, complete_write_item v) :: _ => v
-  | _ :: t' => write_version t'
+  | (_, complete_write_item a' v) :: t' =>
+    if Nat.eq_dec a a' then v else write_version a t'
+  | _ :: t' => write_version a t'
   | [] => 0
   end.
 
-Fixpoint trace_tid_last_write tid t: option value :=
+Fixpoint tid_last_write tid a t: option value :=
   match t with
-  | (tid', a) :: t' =>
-    if Nat.eq_dec tid tid'
-    then match a with
-         | write_item v => Some v
-         | complete_write_item _ => None
-         | _ => trace_tid_last_write tid t'
+  | (tid', ac) :: t' =>
+    if Nat.eq_dec tid tid' 
+    then match ac with
+         | write_item a' v =>
+           if Nat.eq_dec a a' then Some v else tid_last_write tid a t'
+         | complete_write_item a' _ =>
+           if Nat.eq_dec a a' then None else tid_last_write tid a t'
+         | _ => tid_last_write tid a t'
          end
-    else trace_tid_last_write tid t'
+    else tid_last_write tid a t'
   | [] => None
   end.
 
-Fixpoint locked_by (t:trace) default : tid :=
+Fixpoint locked_by (a:addr) (t:trace) default : tid :=
   match t with
-  | (tid, lock_write_item) :: _ => tid
-  | (_, unlock_write_item) :: _ => default
-  | (_, complete_write_item _) :: _ => default
-  | _ :: t' => locked_by t' default
+  | (tid, lock_write_item a') :: t' =>
+    if Nat.eq_dec a a' then tid else locked_by a t' default
+  | (_, unlock_write_item a') :: t' =>
+    if Nat.eq_dec a a' then default else locked_by a t' default
+  | (_, complete_write_item a' _) :: t' =>
+    if Nat.eq_dec a a' then default else locked_by a t' default
+  | _ :: t' => locked_by a t' default
   | [] => default
   end.
 
@@ -217,75 +220,75 @@ Inductive sto_trace : trace -> Prop :=
     -> sto_trace t
     -> sto_trace ((tid, start_txn)::t)
 
-| read_item_step: forall t tid,
+| read_item_step: forall tid t ad,
     tid_phase tid t = 1
-    -> locked_by t 0 = 0
+    -> locked_by ad t 0 = 0
     -> sto_trace t
-    -> sto_trace ((tid, read_item (write_version t)) :: t)
+    -> sto_trace ((tid, read_item ad (write_version ad t)) :: t)
 
-| write_item_step: forall t tid val,
+| write_item_step: forall tid t ad val,
     tid_phase tid t = 1
     -> sto_trace t
-    -> sto_trace ((tid, write_item val) :: t)
+    -> sto_trace ((tid, write_item ad val) :: t)
 
-| try_commit_txn_step: forall t tid,
+| try_commit_txn_step: forall tid t,
     tid_phase tid t = 1
     -> sto_trace t
     -> sto_trace ((tid, try_commit_txn)::t)
 
-| lock_write_item_step: forall t tid v,
+| lock_write_item_step: forall tid t ad v,
     tid_phase tid t = 2
-    -> In (tid, write_item v) t
-    -> locked_by t 0 = 0
+    -> In (tid, write_item ad v) t
+    -> locked_by ad t 0 = 0
     -> sto_trace t
-    -> sto_trace ((tid, lock_write_item) :: t)
+    -> sto_trace ((tid, lock_write_item ad) :: t)
 
 (*sequential point*)
-| seq_point_step: forall t tid,
+| seq_point_step: forall tid t,
     tid_phase tid t = 2
-    -> (forall v, In (tid, write_item v) t
-                  -> In (tid, lock_write_item) t)
+    -> (forall ad v, In (tid, write_item ad v) t
+                     -> In (tid, lock_write_item ad) t)
     -> sto_trace t
     -> sto_trace ((tid, seq_point) :: t)
 
-| validate_read_item_step: forall t tid vers,
+| validate_read_item_step: forall tid t ad vers,
     tid_phase tid t = 3
-    -> locked_by t tid = tid (* unlocked or locked by me *)
-    -> write_version t = vers
-    -> In (tid, read_item vers) t (* only validate unvalidated reads we performed *)
-    -> ~ In (tid, validate_read_item vers) t
+    -> locked_by ad t tid = tid (* unlocked or locked by me *)
+    -> write_version ad t = vers
+    -> In (tid, read_item ad vers) t (* only validate unvalidated reads we performed *)
+    -> ~ In (tid, validate_read_item ad vers) t
     -> sto_trace t
-    -> sto_trace ((tid, validate_read_item vers) :: t)
+    -> sto_trace ((tid, validate_read_item ad vers) :: t)
 
-| abort_txn_step: forall t tid,
+| abort_txn_step: forall tid t,
     tid_phase tid t > 0
     -> tid_phase tid t < 4
     -> sto_trace t
     -> sto_trace ((tid, abort_txn) :: t)
 
-| unlock_item_step: forall t tid,
+| unlock_item_step: forall tid t ad,
     tid_phase tid t = 6
-    -> locked_by t 0 = tid
+    -> locked_by ad t 0 = tid
     -> sto_trace t
-    -> sto_trace ((tid, unlock_write_item) :: t)
+    -> sto_trace ((tid, unlock_write_item ad) :: t)
 
-| commit_txn_step: forall t tid,
+| commit_txn_step: forall tid t,
     tid_phase tid t = 3
-    -> (forall vers, In (tid, read_item vers) t
-                     -> In (tid, validate_read_item vers) t)
+    -> (forall ad vers, In (tid, read_item ad vers) t
+                        -> In (tid, validate_read_item ad vers) t)
     -> sto_trace t
     -> sto_trace ((tid, commit_txn) :: t)
 
-| complete_write_item_step: forall t tid val,
+| complete_write_item_step: forall tid t ad val,
     tid_phase tid t = 4
-    -> locked_by t 0 = tid
-    -> trace_tid_last_write tid t = Some val
+    -> locked_by ad t 0 = tid
+    -> tid_last_write tid ad t = Some val
     -> sto_trace t
-    -> sto_trace ((tid, complete_write_item (S (write_version t))) :: t)
+    -> sto_trace ((tid, complete_write_item ad (S (write_version ad t))) :: t)
 
-| commit_done_step: forall t tid,
+| commit_done_step: forall tid t,
     tid_phase tid t = 4
-    -> locked_by t 0 <> tid
+    -> (forall ad, locked_by ad t 0 <> tid)
     -> ~ In (tid, commit_done_txn) t
     -> sto_trace t
     -> sto_trace ((tid, commit_done_txn) :: t).
@@ -316,14 +319,14 @@ Qed.
 
 Lemma phase_increase_head tid a t:
   sto_trace ((tid, a) :: t) ->
-  action_phase a >= tid_phase tid t.
+  tid_phase tid t <= action_phase a.
 Proof.
   intros; inversion H; cbn; omega.
 Qed.
 
 Lemma phase_increase_app tid t1 t2:
   sto_trace (t1 ++ t2) ->
-  tid_phase tid (t1 ++ t2) >= tid_phase tid t2.
+  tid_phase tid t2 <= tid_phase tid (t1 ++ t2).
 Proof.
   induction t1; intros.
   - simpl; omega.
@@ -338,7 +341,7 @@ Qed.
 Lemma phase_increase_in tid a t:
   sto_trace t ->
   In (tid, a) t ->
-  tid_phase tid t >= action_phase a.
+  action_phase a <= tid_phase tid t.
 Proof.
   intros H I; apply in_split in I.
   destruct I as [l1 [l2 L]].
@@ -351,7 +354,7 @@ Qed.
 Lemma phase_increase_in_app tid a (t1 t2:trace):
   sto_trace (t1 ++ t2) ->
   In (tid, a) (t1 ++ t2) ->
-  action_phase a > tid_phase tid t2 ->
+  tid_phase tid t2 < action_phase a ->
   In (tid, a) t1.
 Proof.
   intros T I A.
@@ -437,26 +440,30 @@ Qed.
 
 (** Facts about versions *)
 
-Lemma write_version_increase_app t1 t2:
+Lemma write_version_increase_app ad t1 t2:
   sto_trace (t1 ++ t2) ->
-  write_version t2 <= write_version (t1 ++ t2).
+  write_version ad t2 <= write_version ad (t1 ++ t2).
 Proof.
   induction t1; intros T.
   cbn; omega.
   destruct a; inversion T; rewrite <- H0 in *; clear H0.
   all: cbn; auto.
+  destruct (Nat.eq_dec ad ad0); auto.
+  rewrite <- e in *; clear e; auto.
 Qed.
 
-Lemma read_version_increase_in tid v t:
+Lemma read_version_increase_in tid ad v t:
   sto_trace t ->
-  In (tid, read_item v) t ->
-  v <= write_version t.
+  In (tid, read_item ad v) t ->
+  v <= write_version ad t.
 Proof.
   intros T; induction T; intros I.
   destruct I.
-  all: destruct I as [I | I]; try congruence.
+  all: destruct I as [I|I]; try congruence.
   all: cbn; auto.
   inversion I; omega.
+  destruct (Nat.eq_dec ad ad0); auto.
+  rewrite <- e in *; clear e; auto.
 Qed.
 
 
@@ -506,16 +513,16 @@ Proof.
   cbn; destruct (Nat.eq_dec tid' t0); [ subst; contradiction | auto ].
 Qed.
 
-Lemma remove_tid_write_version tid t:
+Lemma remove_tid_write_version tid ad t:
   sto_trace t ->
   tid_phase tid t <> 4 ->
-  write_version (remove_tid tid t) = write_version t.
+  write_version ad (remove_tid tid t) = write_version ad t.
 Proof.
   intros T; induction T; intros P; cbn in *; auto.
-  all: destruct (Nat.eq_dec tid tid0); [ rewrite e in * | ].
+  all: destruct (Nat.eq_dec tid tid0); [ rewrite e in *; clear e | ].
   all: try solve [ apply IHT; omega ].
   contradiction.
-  now cbn.
+  cbn; destruct (Nat.eq_dec ad ad0); auto.
 Qed.
 
 Lemma remove_tid_zero t:
@@ -533,9 +540,9 @@ Proof.
   now rewrite (IHt H1).
 Qed.
 
-Lemma remove_tid_last_write tid tid' t:
+Lemma remove_tid_last_write tid tid' ad t:
   tid <> tid' ->
-  trace_tid_last_write tid' (remove_tid tid t) = trace_tid_last_write tid' t.
+  tid_last_write tid' ad (remove_tid tid t) = tid_last_write tid' ad t.
 Proof.
   induction t; intros N; cbn in *; auto.
   destruct a; destruct a;
@@ -543,94 +550,102 @@ Proof.
       cbn; auto.
   all: try congruence.
   all: destruct (Nat.eq_dec tid' t0); try congruence; auto.
+  all: destruct (Nat.eq_dec ad ad0); auto.
 Qed.
 
 
 (** Facts about [locked_by] *)
 
-Lemma locked_by_unlocked_in tid t:
+Lemma locked_by_unlocked_in tid ad t:
   (forall x, In x t -> fst x > 0) ->
-  locked_by t 0 = 0 ->
-  locked_by t tid = tid.
+  locked_by ad t 0 = 0 ->
+  locked_by ad t tid = tid.
 Proof.
   induction t; intros A L; cbn in *; auto.
   destruct a; destruct a.
   all: try solve [ apply IHt; auto ].
+  all: destruct (Nat.eq_dec ad ad0); auto.
+  rewrite <- e in *; clear e.
   assert (n > 0). {
-    replace n with (fst (n, lock_write_item)).
+    replace n with (fst (n, lock_write_item ad)).
     apply A; now left.
     now simpl.
   }
   omega.
-  all: reflexivity.
 Qed.
 
-Lemma locked_by_unlocked tid t:
+Lemma locked_by_unlocked tid ad t:
   sto_trace t ->
-  locked_by t 0 = 0 ->
-  locked_by t tid = tid.
+  locked_by ad t 0 = 0 ->
+  locked_by ad t tid = tid.
 Proof.
   intros T L; apply locked_by_unlocked_in; auto.
   intros x I; destruct x; simpl.
   now apply (trace_in_nonzero _ a t).
 Qed.
 
-Lemma locked_by_self tid t:
+Lemma locked_by_self tid ad t:
   sto_trace t ->
-  locked_by t 0 = tid ->
-  locked_by t tid = tid.
+  locked_by ad t 0 = tid ->
+  locked_by ad t tid = tid.
 Proof.
   intros T; induction T; cbn in *; intros L; auto.
+  all: destruct (Nat.eq_dec ad ad0); auto.
 Qed.
 
-Lemma locked_by_self_or tid t:
-  locked_by t tid = tid ->
-  locked_by t 0 = 0 \/ locked_by t 0 = tid.
+Lemma locked_by_self_or tid ad t:
+  locked_by ad t tid = tid ->
+  locked_by ad t 0 = 0 \/ locked_by ad t 0 = tid.
 Proof.
   induction t; cbn in *; intros.
   now left.
   destruct a; destruct a; try solve [ now apply IHt ].
-  all: intuition.
+  all: destruct (Nat.eq_dec ad ad0); auto.
 Qed.
 
-Lemma locked_by_or tid tid' t:
-  locked_by t tid = locked_by t tid' \/ locked_by t 0 = 0.
+Lemma locked_by_or tid tid' ad t:
+  locked_by ad t tid = locked_by ad t tid' \/ locked_by ad t 0 = 0.
 Proof.
   induction t; cbn in *; intros.
   now right.
   destruct a; destruct a; auto.
+  all: destruct (Nat.eq_dec ad ad0); auto.
 Qed.
 
-Lemma locked_by_other tid tid' t:
+Lemma locked_by_other tid tid' ad t:
   sto_trace t ->
   tid' > 0 ->
-  locked_by t 0 = tid' ->
-  locked_by t tid = tid'.
+  locked_by ad t 0 = tid' ->
+  locked_by ad t tid = tid'.
 Proof.
   intros T; induction T; cbn in *; intros N L; auto.
+  omega.
+  all: destruct (Nat.eq_dec ad ad0); auto.
   all: omega.
 Qed.
 
-Lemma remove_tid_locked_by_neq tid tid' t:
+Lemma remove_tid_locked_by_neq tid tid' ad t:
   sto_trace t ->
-  locked_by t tid <> tid ->
-  locked_by (remove_tid tid t) tid' = locked_by t tid'.
+  locked_by ad t tid <> tid ->
+  locked_by ad (remove_tid tid t) tid' = locked_by ad t tid'.
 Proof.
   intros T; induction T; intros L; cbn in *; auto.
   all: destruct (Nat.eq_dec tid tid0); auto.
-  all: congruence.
+  all: cbn; destruct (Nat.eq_dec ad ad0); auto.
+  all: try congruence.
 Qed.
 
-Lemma remove_tid_locked_by_eq tid tid' t:
+Lemma remove_tid_locked_by_eq tid tid' ad t:
   sto_trace t ->
-  locked_by t tid = tid ->
-  locked_by (remove_tid tid t) tid' = tid'.
+  locked_by ad t tid = tid ->
+  locked_by ad (remove_tid tid t) tid' = tid'.
 Proof.
   intros T; induction T; intros L; cbn in *; auto.
   all: destruct (Nat.eq_dec tid tid0); auto.
+  all: cbn in *; destruct (Nat.eq_dec ad ad0); auto.
   apply IHT; apply locked_by_unlocked; auto.
-  congruence.
-  all: apply IHT; apply locked_by_self; auto; now rewrite e.
+  all: try congruence.
+  all: apply IHT; apply locked_by_self; subst; auto.
 Qed.
 
 
@@ -658,25 +673,26 @@ Qed.
 
 
 
-Lemma track_lock_cons tid tid' t a:
+Lemma track_lock_cons tid tid' ad t a:
   sto_trace ((tid', a) :: t) ->
-  locked_by t 0 = tid ->
-  locked_by ((tid', a) :: t) 0 = tid
-  \/ tid = 0 /\ a = lock_write_item
-  \/ tid = tid' /\ a = unlock_write_item
-  \/ tid = tid' /\ exists val, a = complete_write_item val.
+  locked_by ad t 0 = tid ->
+  locked_by ad ((tid', a) :: t) 0 = tid
+  \/ tid = 0 /\ a = lock_write_item ad
+  \/ tid = tid' /\ a = unlock_write_item ad
+  \/ tid = tid' /\ exists val, a = complete_write_item ad val.
 Proof.
   intros T L.
   assert (tid' > 0) as TG. {
     apply trace_in_nonzero with (a:=a) (t:=(tid', a)::t); cbn; auto.
   }
   inversion T; subst; cbn; auto.
+  all: destruct (Nat.eq_dec ad ad0); cbn; subst; auto.
   right; right; right; eauto.
 Qed.
 
-Lemma locked_phase tid t:
+Lemma locked_phase tid ad t:
   sto_trace t ->
-  locked_by t 0 = tid ->
+  locked_by ad t 0 = tid ->
   tid > 0 ->
   tid_phase tid t >= 2.
 Proof.
@@ -686,7 +702,7 @@ Proof.
   all: destruct (Nat.eq_dec tid tid0); try omega.
   all: try (now apply IHT).
   1-3: subst; apply IHT in e; omega.
-  1-3: simpl in L; omega.
+  1-3: cbn in L; destruct (Nat.eq_dec ad ad0); auto; omega.
 Qed.
 
 Lemma commit_phase_cons tid p t:
@@ -736,63 +752,60 @@ Proof.
 Qed.
 
 
-Lemma phase_2_preserves_lock tid t1 t2:
+Lemma phase_2_preserves_lock tid ad t1 t2:
   sto_trace (t1 ++ t2) ->
   tid_phase tid (t1 ++ t2) = 2 ->
-  locked_by t2 0 = tid ->
-  locked_by (t1 ++ t2) 0 = tid.
+  locked_by ad t2 0 = tid ->
+  locked_by ad (t1 ++ t2) 0 = tid.
 Proof.
   revert t2.
   induction t1; intros t2 T P L.
   now cbn.
   destruct a as [tid' a].
   cbn in P; destruct (Nat.eq_dec tid tid').
-  - destruct a; simpl in *; try omega.
-    + rewrite e in *; clear e tid.
-      assert (tid_phase tid' t2 >= 2). {
-        apply locked_phase.
-        now apply trace_app with (t1:=(tid',try_commit_txn)::t1).
-        auto.
-        apply trace_in_nonzero with (a:=try_commit_txn) (t:=(tid', try_commit_txn)::t1 ++ t2).
-        auto.
-        simpl; now left.
-      }
-      inversion T; subst.
-      apply (phase_increase_app (locked_by t2 0)) in H3; omega.
-    + auto.
-  - assert (locked_by (t1 ++ t2) 0 = tid) as LA. {
+  - rewrite <- e in *; clear tid' e.
+    rewrite <- app_comm_cons in *.
+    inversion T; rewrite <- H0 in P; cbn in P; try omega.
+    apply locked_phase in L.
+    assert (tid_phase tid t2 <= 1). {
+      rewrite <- H1; apply phase_increase_app; auto.
+    }
+    omega.
+    now apply trace_app in H3.
+    apply trace_phase_nonzero with (t:=t1 ++ t2); auto; omega.
+    cbn; destruct (Nat.eq_dec ad ad0); auto.
+  - assert (locked_by ad (t1 ++ t2) 0 = tid) as LA. {
       apply IHt1; auto.
       now apply (trace_cons _ _ T).
     }
-    clear IHt1 L.
-
     assert (tid > 0). {
       apply trace_phase_nonzero with (t:=t1++t2).
-      now apply trace_cons with (ta:=(tid',a)).
+      now apply (trace_cons _ _ T).
       omega.
     }
-
-    inversion T; cbn in *; auto; omega.
+    all: cbn in *; inversion T; auto.
+    all: destruct (Nat.eq_dec ad ad0); auto.
+    all: rewrite <- e in *; clear ad0 e; rewrite LA in *; omega.
 Qed.
 
-Lemma locked_at_seq_point tid t1 t2 v:
-  sto_trace ((tid, seq_point) :: t1 ++ (tid, write_item v) :: t2) ->
-  locked_by (t1 ++ (tid, write_item v) :: t2) 0 = tid.
+Lemma locked_at_seq_point tid t1 t2 ad v:
+  sto_trace ((tid, seq_point) :: t1 ++ (tid, write_item ad v) :: t2) ->
+  locked_by ad (t1 ++ (tid, write_item ad v) :: t2) 0 = tid.
 Proof.
   intros T.
   inversion T.
   assert (tid > 0) as TG. {
-    apply trace_in_nonzero with (a:=write_item v) (t:=t); rewrite H0; auto.
+    apply trace_in_nonzero with (a:=write_item ad v) (t:=t); rewrite H0; auto.
     apply in_or_app; right; now left.
   }
 
-  assert (In (tid, lock_write_item) t1). {
-    assert (In (tid, lock_write_item) t). {
+  assert (In (tid, lock_write_item ad) t1). {
+    assert (In (tid, lock_write_item ad) t). {
       rewrite H0.
       apply H2 with (v0:=v).
       apply in_or_app; cbn; intuition.
     }
-    apply phase_increase_in_app with (t2:=(tid, write_item v) :: t2); auto.
+    apply phase_increase_in_app with (t2:=(tid, write_item ad v) :: t2); auto.
     now rewrite <- H0.
     simpl; destruct (Nat.eq_dec tid tid); intuition.
   }
@@ -802,13 +815,15 @@ Proof.
   subst.
   repeat rewrite <- app_assoc in *.
   repeat rewrite <- app_comm_cons in *.
-  remember ((tid, lock_write_item) :: t1b ++ (tid, write_item v) :: t2) as tx.
-  assert (locked_by tx 0 = tid). {
-    rewrite Heqtx; now cbn.
+  remember ((tid, lock_write_item ad) :: t1b ++ (tid, write_item ad v) :: t2) as tx.
+  assert (locked_by ad tx 0 = tid). {
+    rewrite Heqtx.
+    cbn.
+    destruct (Nat.eq_dec ad ad); congruence.
   }
   assert (tid_phase tid tx = 2). {
     assert (tid_phase tid tx >= 2). {
-      apply locked_phase; auto.
+      apply locked_phase with (ad:=ad); auto.
       now apply trace_app with (t1:=t1a).
     }
     assert (2 >= tid_phase tid tx). {
@@ -823,7 +838,7 @@ Qed.
 
 Lemma seq_point_after t1 t2 tid action:
   sto_trace ((tid, action) :: t1 ++ (tid, commit_txn) :: t2)
-  -> action = complete_write_item (S (write_version t2))
+  -> (exists ad, action = complete_write_item ad (S (write_version ad t2)))
      \/ action = commit_done_txn.
 Proof.
   intros T.
@@ -836,15 +851,16 @@ Proof.
   2: now right.
   left.
 
-  assert (write_version (t1 ++ (tid, commit_txn) :: t2) =
-          write_version t2). {
+  exists ad.
+  assert (write_version ad (t1 ++ (tid, commit_txn) :: t2) =
+          write_version ad t2). {
     subst.
     clear TG4 val H2 H3 H4 H5.
-    inversion T; subst; clear T H4 val.
+    inversion T; subst.
+    clear T H5 val H1.
     remember (t1 ++ (tid, commit_txn) :: t2) as t.
-    clear H0.
-    revert t1 t2 tid Heqt H2 H3.
-    induction H5; intros t1 t2 tid T P L.
+    revert t1 t2 tid Heqt H3 H4.
+    induction H6; intros t1 t2 tid T P L.
     all: destruct t1; simpl in T.
     1,2: congruence.
     all: inversion T.
@@ -856,22 +872,24 @@ Proof.
          end.
     all: try solve [ rewrite <- Teq; apply (IHsto_trace _ _ _ Teq); auto ].
     all: assert (tid > 0)
-      by (apply (trace_in_nonzero _ commit_txn _ H5);
+      by (apply (trace_in_nonzero _ commit_txn _ H6);
           rewrite Teq; apply in_or_app; right; now left).
-    all: try omega.
-
-    rewrite <- Teq; apply (IHsto_trace _ _ _ Teq); auto.
-    rewrite Teq; apply commit_phase_app.
-    rewrite <- Teq; auto.
-    cbn; destruct (Nat.eq_dec tid tid); congruence.
+    all: try (destruct (Nat.eq_dec ad ad0); [ omega | ]).
+    1,2,4,5: rewrite <- Teq; apply (IHsto_trace _ _ _ Teq); auto.
+    all: rewrite <- e in *; clear tid0 e; auto.
+    assert (action_phase commit_txn <= tid_phase tid t). {
+      apply phase_increase_in; auto.
+      rewrite Teq; apply in_or_app; right; now left.
+    }
+    cbn in H3; omega.
   }
 
   now rewrite H6.
 Qed.
 
-Lemma unlocked_after_commit_done tid t1 t2:
+Lemma unlocked_after_commit_done tid ad t1 t2:
   sto_trace (t1 ++ (tid, commit_done_txn) :: t2) ->
-  locked_by (t1 ++ (tid, commit_done_txn) :: t2) 0 <> tid.
+  locked_by ad (t1 ++ (tid, commit_done_txn) :: t2) 0 <> tid.
 Proof.
   intros T.
   assert (tid > 0) as G. {
@@ -882,14 +900,15 @@ Proof.
   inversion T; auto.
   destruct a; destruct a.
   all: try solve [ apply IHt1; now apply trace_cons in T ].
-  2, 3: omega.
-  assert (tid_phase tid (t1 ++ (tid, commit_done_txn) :: t2) = 4) as P4. {
-    apply commit_phase_app; auto.
-    now apply trace_cons in T.
-    cbn; destruct (Nat.eq_dec tid tid); congruence.
-  }
+  all: destruct (Nat.eq_dec ad ad0); auto.
+  2,3,4: apply IHt1; apply (trace_cons _ _ T).
   inversion T.
-  destruct (Nat.eq_dec t tid); try congruence.
+  assert (4 <= tid_phase tid (t1 ++ (tid, commit_done_txn) :: t2)). {
+    replace 4 with (action_phase commit_done_txn) by (now cbn).
+    apply phase_increase_in; auto.
+    apply in_or_app; right; now left.
+  }
+  intros F; rewrite <- F in *; omega.
 Qed.
 
 Lemma no_steps_after_commit_done tid tid' a t1 t2:
@@ -907,7 +926,7 @@ Proof.
   all: destruct (Nat.eq_dec tid tid'); auto.
   all: rewrite <- e in *; clear e.
   - omega.
-  - assert (locked_by t 0 <> tid). {
+  - assert (locked_by ad t 0 <> tid). {
       rewrite Heqt in *; now apply unlocked_after_commit_done.
     }
     congruence.
@@ -973,7 +992,7 @@ Proof.
            [ constructor; auto; rewrite (remove_tid_phase _ _ _ n); auto ].
 
   {
-    rewrite <- (remove_tid_write_version _ _ T P); constructor.
+    rewrite <- (remove_tid_write_version _ _ _ T P); constructor.
     now rewrite remove_tid_phase.
     rewrite remove_tid_locked_by_eq; auto; now apply locked_by_unlocked.
     auto.
@@ -990,9 +1009,9 @@ Proof.
   {
     constructor.
     rewrite (remove_tid_phase _ _ _ n); auto.
-    intros v I.
+    intros ad v I.
     apply in_remove_tid; auto.
-    apply (H0 v).
+    apply (H0 ad v).
     apply (remove_tid_in _ _ _ I).
     auto.
   }
@@ -1000,7 +1019,7 @@ Proof.
   {
     constructor.
     rewrite (remove_tid_phase _ _ _ n); auto.
-    destruct (Nat.eq_dec (locked_by t tid) tid);
+    destruct (Nat.eq_dec (locked_by ad t tid) tid);
       [ rewrite remove_tid_locked_by_eq | rewrite remove_tid_locked_by_neq ];
       auto.
     rewrite remove_tid_write_version; auto.
@@ -1013,7 +1032,7 @@ Proof.
   {
     constructor.
     rewrite (remove_tid_phase _ _ _ n); auto.
-    assert (locked_by t tid <> tid). {
+    assert (locked_by ad t tid <> tid). {
       rewrite locked_by_other with (tid':=tid0); auto.
       apply trace_phase_nonzero with (t:=t); auto; omega.
     }
@@ -1024,7 +1043,7 @@ Proof.
   {
     constructor.
     rewrite (remove_tid_phase _ _ _ n); auto.
-    intros vers I.
+    intros ad vers I.
     apply in_remove_tid; auto.
     apply H0.
     apply (remove_tid_in tid); auto.
@@ -1032,10 +1051,10 @@ Proof.
   }
 
   {
-    rewrite <- (remove_tid_write_version _ _ T P).
+    rewrite <- (remove_tid_write_version _ _ _ T P).
     apply complete_write_item_step with (val:=val).
     now rewrite remove_tid_phase.
-    assert (locked_by t tid <> tid). {
+    assert (locked_by ad t tid <> tid). {
       rewrite locked_by_other with (tid':=tid0); auto.
       apply trace_phase_nonzero with (t:=t); auto; omega.
     }
@@ -1047,7 +1066,8 @@ Proof.
   {
     constructor.
     now rewrite remove_tid_phase.
-    destruct (Nat.eq_dec (locked_by t tid) tid);
+    intros ad;
+    destruct (Nat.eq_dec (locked_by ad t tid) tid);
       [ rewrite remove_tid_locked_by_eq | rewrite remove_tid_locked_by_neq ];
       auto.
     assert (tid0 > 0). {
@@ -1070,10 +1090,10 @@ Proof.
   destruct a; destruct (Nat.eq_dec tid n); auto.
 Qed.
 
-Lemma write_version_swap t1 t2 tid1 tid2 a1 a2:
+Lemma write_version_swap t1 t2 ad tid1 tid2 a1 a2:
   action_phase a1 < 4 ->
-  write_version (t1 ++ (tid2, a2) :: (tid1, a1) :: t2) =
-  write_version (t1 ++ (tid1, a1) :: (tid2, a2) :: t2).
+  write_version ad (t1 ++ (tid2, a2) :: (tid1, a1) :: t2) =
+  write_version ad (t1 ++ (tid1, a1) :: (tid2, a2) :: t2).
 Proof.
   induction t1; intros AP; cbn in *.
 
@@ -1082,16 +1102,16 @@ Proof.
   all: destruct a; repeat rewrite (IHt1 AP); auto.
 Qed.
 
-Lemma locked_by_swap_head t1 t2 tid1 tid2 a1 a2 tid:
-  locked_by ((tid2, a2) :: (tid1, a1) :: t2) tid =
-  locked_by ((tid1, a1) :: (tid2, a2) :: t2) tid ->
-  locked_by (t1 ++ (tid2, a2) :: (tid1, a1) :: t2) tid =
-  locked_by (t1 ++ (tid1, a1) :: (tid2, a2) :: t2) tid.
+Lemma locked_by_swap_head t1 t2 ad tid1 tid2 a1 a2 tid:
+  locked_by ad ((tid2, a2) :: (tid1, a1) :: t2) tid =
+  locked_by ad ((tid1, a1) :: (tid2, a2) :: t2) tid ->
+  locked_by ad (t1 ++ (tid2, a2) :: (tid1, a1) :: t2) tid =
+  locked_by ad (t1 ++ (tid1, a1) :: (tid2, a2) :: t2) tid.
 Proof.
   induction t1; cbn; auto.
   intros; destruct a; destruct a.
   all: try solve [now apply IHt1].
-  all: congruence.
+  all: destruct (Nat.eq_dec ad ad0); auto.
 Qed.
 
 Lemma in_middle_swap_iff {A:Type} (t1 t2:list A) p1 p2 p:
@@ -1106,30 +1126,40 @@ Qed.
 
 Definition action_internal a :=
   match a with
-  | read_item _
-  | validate_read_item _
-  | lock_write_item
-  | complete_write_item _
-  | unlock_write_item => False
+  | read_item _ _
+  | validate_read_item _ _
+  | lock_write_item _
+  | complete_write_item _ _
+  | unlock_write_item _ => False
   | _ => True
   end.
 
-Definition action_commute_read a :=
+Definition action_commute_read ad a :=
   match a with
-  | lock_write_item
-  | complete_write_item _
-  | unlock_write_item => False
+  | lock_write_item ad'
+  | complete_write_item ad' _
+  | unlock_write_item ad' => ad <> ad'
   | _ => True
   end.
 
 Local Ltac check_action :=
   match goal with
   | [ H: action_internal ?a, H2: ?b = ?a |- _ ] =>
-    rewrite <- H2 in *; clear H2; cbn in H; try contradiction; clear H
-  | [ H: action_commute_read ?a, H2: ?b = ?a |- _ ] =>
-    rewrite <- H2 in *; clear H2; cbn in H; try contradiction; clear H
+    (tryif is_var a then rewrite <- H2 in *; clear H2 else idtac);
+    cbn in H; try contradiction; clear H
+  | [ H: action_commute_read ?ad ?a, H2: ?b = ?a |- _ ] =>
+    (tryif is_var a then rewrite <- H2 in *; clear H2 else idtac);
+    cbn in H; try contradiction
   | [ H: action_phase ?a < _, H2: ?b = ?a |- _ ] =>
-    rewrite <- H2 in *; clear H2; cbn in H; try omega
+    (tryif is_var a then rewrite <- H2 in *; clear H2 else idtac);
+    cbn in H; try omega
+  | [ H: action_phase ?a < _ |- _ ] =>
+    cbn in H; try omega
+  | [ H: _ <= action_phase ?a, H2: ?b = ?a |- _ ] =>
+    (tryif is_var a then rewrite <- H2 in *; clear H2 else idtac);
+    cbn in H; try omega
+  | [ H: _ <= action_phase ?a |- _ ] =>
+    cbn in H; try omega
   end.
 Local Ltac fix_phase :=
   match goal with
@@ -1137,59 +1167,81 @@ Local Ltac fix_phase :=
       |- context [ tid_phase ?tid ?x ] ] => now rewrite TP
   | [ TP: tid_phase ?tid _ = tid_phase ?tid ?x
       |- context [ tid_phase ?tid ?x ] ] => now rewrite <- TP
-  | [ L: locked_by ?t ?a = ?x
-      |- locked_by (_ :: ?t) ?a = ?x ] => cbn; apply L
-  | [ L: locked_by ?t ?a <> ?x
-      |- locked_by (_ :: ?t) ?a <> ?x ] => cbn; apply L
-  | [ L: locked_by (_ :: ?t) ?a = ?x
-      |- locked_by ?t ?a = ?x ] => cbn in L; apply L
-  | [ WV: write_version ?t = ?x
-      |- write_version (_ :: ?t) = ?x ] => cbn; apply WV
-  | [ LW: trace_tid_last_write ?tid ?t = ?x
-      |- trace_tid_last_write ?tid ((?tid2, ?a) :: ?t) = ?x ] =>
+  | [ L: context [ locked_by ?ad ?t ?a = ?x ]
+      |- locked_by ?ad (_ :: ?t) ?a = ?x ] => cbn; apply L
+  | [ L: context [ locked_by ?ad ?t ?a <> ?x ]
+      |- locked_by ?ad (_ :: ?t) ?a <> ?x ] => cbn; apply L
+  | [ L: context [ locked_by ?ad (?c ?ad1 :: ?t) ?a = ?x ],
+      N: ?ad <> ?ad1 |- locked_by ?ad ?t ?a = ?x ] =>
+    cbn in L; 
+    let X := fresh in
+    destruct (Nat.eq_dec ad ad1) as [X|X];
+    [ congruence | ]; clear X; apply L
+  | [ L: context [ locked_by ?ad (_ :: ?t) ?a = ?x ]
+      |- locked_by ?ad ?t ?a = ?x ] => cbn in L; apply L
+  | [ L : forall _, locked_by _ ?t ?a = ?x
+      |- forall _, locked_by _ ?t ?a = ?x ] =>
+      let ad := fresh in intros ad; cbn; apply L
+  | [ L : forall _, locked_by _ ?t ?a <> ?x
+      |- forall _, locked_by _ ?t ?a <> ?x ] =>
+      let ad := fresh in intros ad; cbn; apply L
+  | [ L : forall _, locked_by _ ?t ?a = ?x
+      |- forall _, locked_by _ (_ :: ?t) ?a = ?x ] =>
+      let ad := fresh in intros ad; cbn; apply L
+  | [ L : forall _, locked_by _ ?t ?a <> ?x
+      |- forall _, locked_by _ (_ :: ?t) ?a <> ?x ] =>
+      let ad := fresh in intros ad; cbn; apply L
+  | [ |- context [ locked_by ?ad ?t ?a ] ] =>
+      intros ad; fix_phase
+  | [ WV: write_version ?ad ?t = ?x
+      |- write_version ?ad (_ :: ?t) = ?x ] => cbn; apply WV
+  | [ LW: tid_last_write ?tid ?ad ?t = ?x
+      |- tid_last_write ?tid ?ad ((?tid2, ?a) :: ?t) = ?x ] =>
     cbn; destruct (Nat.eq_dec tid tid2); [ congruence | apply LW ]
-  | [ LW: trace_tid_last_write ?tid ((?tid2, ?a) :: ?t) = ?x
-      |- trace_tid_last_write ?tid ?t = ?x ] =>
+  | [ LW: tid_last_write ?tid ?ad ((?tid2, ?a) :: ?t) = ?x
+      |- tid_last_write ?tid ?ad ?t = ?x ] =>
     cbn in LW; destruct (Nat.eq_dec tid tid2); [ congruence | apply LW ]
   | [ H: In ?p ?t
       |- In ?p (_ :: ?t) ] => right; apply H
   | [ H: In ?p (_ :: ?t)
       |- In ?p ?t ] => destruct H; [ congruence | apply H ]
   | [ |- context [ In (?tid, _) _ ] ] =>
+    let ad := fresh in
     let vx := fresh in
     let I := fresh in
-    intros vx I; destruct I; [ congruence | right; revert vx I; assumption ]
+    intros ad vx I; destruct I; [ congruence | right; revert ad vx I; assumption ]
   | [ H: ~ In ?p ?t
       |- ~ In ?p (?x :: ?t) ] => contradict H; destruct H; [ congruence | assumption ]
   | [ H: ~ In ?p (?x :: ?t)
       |- ~ In ?p ?t ] => contradict H; right; assumption
   | [ |- sto_trace ((?tid, start_txn) :: ?t) ] =>
     constructor; [ fix_phase | assumption | auto ]
-  | [ |- sto_trace ((?tid, read_item _) :: ?t) ] =>
+  | [ |- sto_trace ((?tid, read_item _ _) :: ?t) ] =>
     constructor; [ fix_phase .. | assumption ]
-  | [ |- sto_trace ((?tid, write_item _) :: ?t) ] =>
+  | [ |- sto_trace ((?tid, write_item _ _) :: ?t) ] =>
     constructor; [ fix_phase | assumption ]
   | [ |- sto_trace ((?tid, try_commit_txn) :: ?t) ] =>
     constructor; [ fix_phase | assumption ]
-  | [ H: In (?tid, write_item ?vv) _
-      |- sto_trace ((?tid, lock_write_item) :: ?t) ] =>
+  | [ H: In (?tid, write_item ?ad ?vv) _
+      |- sto_trace ((?tid, lock_write_item ?ad) :: ?t) ] =>
     apply lock_write_item_step with (v:=vv); [ fix_phase .. | assumption ]
   | [ |- sto_trace ((?tid, seq_point) :: ?t) ] =>
     constructor; [ fix_phase | | assumption ]
-  | [ |- sto_trace ((?tid, validate_read_item _) :: ?t) ] =>
+  | [ |- sto_trace ((?tid, validate_read_item _ _) :: ?t) ] =>
     constructor; [ fix_phase .. | assumption ]
   | [ |- sto_trace ((?tid, abort_txn) :: ?t) ] =>
     constructor; [ fix_phase .. | assumption ]
-  | [ |- sto_trace ((?tid, unlock_write_item) :: ?t) ] =>
+  | [ |- sto_trace ((?tid, unlock_write_item _) :: ?t) ] =>
     constructor; [ fix_phase .. | assumption ]
   | [ |- sto_trace ((?tid, commit_txn) :: ?t) ] =>
     constructor; [ fix_phase .. | | assumption ]
-  | [ H: trace_tid_last_write ?tid _ = Some ?vx
-      |- sto_trace ((?tid, complete_write_item (S (write_version ?t))) :: ?t) ] =>
-    apply complete_write_item_step with (val:=vx); [ fix_phase .. | assumption ]
+  | [ LW: tid_last_write ?tid ?ad _ = Some ?vx
+      |- sto_trace ((?tid, complete_write_item ?ad (S (write_version ?ad ?t))) :: ?t) ] =>
+    apply complete_write_item_step with (val:=vx);
+    [ fix_phase .. | assumption ]
   | [ |- sto_trace ((?tid, commit_done_txn) :: ?t) ] =>
     constructor; [ fix_phase .. | assumption ]
-  | [ |- write_version ?t = write_version (?p :: ?t) ] =>
+  | [ |- write_version ?ad ?t = write_version ?ad (?p :: ?t) ] =>
     cbn; reflexivity
   | [ H: In ?p (?a :: ?t) |- In ?p ?t ] =>
     destruct H; [ congruence | assumption ]
@@ -1201,34 +1253,79 @@ Local Ltac chomp1 :=
   match goal with
   | [ |- sto_trace ((?tid, start_txn) :: _ :: _) ] =>
     constructor; [ | assumption | ]; fix_phase
-  | [ |- sto_trace ((?tid, read_item (write_version ?t)) :: ?p :: ?t) ] =>
-    replace (write_version t) with (write_version (p :: t)) by (now cbn);
+  | [ |- sto_trace ((?tid, read_item ?ad (write_version ?ad ?t)) :: ?p :: ?t) ] =>
+    replace (write_version ad t) with (write_version ad (p :: t)) by (now cbn);
     constructor; fix_phase
-  | [ |- sto_trace ((?tid, write_item _) :: _ :: _) ] =>
+  | [ |- sto_trace ((?tid, write_item _ _) :: _ :: _) ] =>
     constructor; fix_phase
   | [ |- sto_trace ((?tid, try_commit_txn) :: _ :: _) ] =>
     constructor; fix_phase
-  | [ H: In (?tid, write_item ?vv) _
-      |- sto_trace ((?tid, lock_write_item) :: _ :: _) ] =>
+  | [ H: In (?tid, write_item ?ad ?vv) _
+      |- sto_trace ((?tid, lock_write_item ?ad) :: _ :: _) ] =>
     apply lock_write_item_step with (v:=vv); fix_phase
   | [ |- sto_trace ((?tid, seq_point) :: _ :: _) ] =>
     constructor; fix_phase
-  | [ |- sto_trace ((?tid, validate_read_item ?vers) :: _ :: _) ] =>
+  | [ |- sto_trace ((?tid, validate_read_item ?ad ?vers) :: _ :: _) ] =>
     constructor; fix_phase
   | [ |- sto_trace ((?tid, abort_txn) :: _ :: _) ] =>
     constructor; fix_phase
-  | [ |- sto_trace ((?tid, unlock_write_item) :: _ :: _) ] =>
+  | [ |- sto_trace ((?tid, unlock_write_item ?ad) :: _ :: _) ] =>
     constructor; fix_phase
   | [ |- sto_trace ((?tid, commit_txn) :: _ :: _) ] =>
     constructor; fix_phase
-  | [ H: trace_tid_last_write ?tid _ = Some ?vx
-      |- sto_trace ((?tid, complete_write_item (S (write_version ?t))) :: ?p :: ?t) ] =>
-    replace (write_version t) with (write_version (p :: t)) by (now cbn);
+  | [ H: tid_last_write ?tid ?ad _ = Some ?vx
+      |- sto_trace ((?tid, complete_write_item ?ad (S (write_version ?ad ?t))) :: ?p :: ?t) ] =>
+    replace (write_version ad t) with (write_version ad (p :: t)) by (now cbn);
     apply complete_write_item_step with (val:=vx); fix_phase
   | [ |- sto_trace ((?tid, commit_done_txn) :: _ :: _) ] =>
     constructor; fix_phase
   end.
 
+Ltac cln :=
+  match goal with
+  | [ |- context [ Nat.eq_dec ?a ?a ] ] =>
+    let X := fresh in
+    destruct (Nat.eq_dec a a) as [X|X]; [ | congruence ]; clear X
+  | [ H : context [ Nat.eq_dec ?a ?a ] |- _ ] =>
+    let X := fresh in
+    destruct (Nat.eq_dec a a) as [X|X]; [ | congruence ]; clear X
+  | [ H : ?a = ?b |- context [ Nat.eq_dec ?a ?b ] ] =>
+    let X := fresh in
+    destruct (Nat.eq_dec a b) as [X|X]; [ | congruence ]; clear X
+  | [ H : ?a = ?b, P : context [ Nat.eq_dec ?a ?b ] |- _ ] =>
+    let X := fresh in
+    destruct (Nat.eq_dec a b) as [X|X]; [ | congruence ]; clear X
+  | [ H : ?a <> ?b |- context [ Nat.eq_dec ?a ?b ] ] =>
+    let X := fresh in
+    destruct (Nat.eq_dec a b) as [X|X]; [ congruence | ]; clear X
+  | [ H : ?a <> ?b, P : context [ Nat.eq_dec ?a ?b ] |- _ ] =>
+    let X := fresh in
+    destruct (Nat.eq_dec a b) as [X|X]; [ congruence | ]; clear X
+  | [ H : ?a = ?b |- context [ Nat.eq_dec ?b ?a ] ] =>
+    let X := fresh in
+    destruct (Nat.eq_dec b a) as [X|X]; [ | congruence ]; clear X
+  | [ H : ?a = ?b, P : context [ Nat.eq_dec ?b ?a ] |- _ ] =>
+    let X := fresh in
+    destruct (Nat.eq_dec b a) as [X|X]; [ | congruence ]; clear X
+  | [ H : ?a <> ?b |- context [ Nat.eq_dec ?b ?a ] ] =>
+    let X := fresh in
+    destruct (Nat.eq_dec b a) as [X|X]; [ congruence | ]; clear X
+  | [ H : ?a <> ?b, P : context [ Nat.eq_dec ?b ?a ] |- _ ] =>
+    let X := fresh in
+    destruct (Nat.eq_dec b a) as [X|X]; [ congruence | ]; clear X
+  | [ H : ?a <= ?b |- context [ ?a <=? ?b ] ] =>
+    rewrite (leb_correct _ _ H)
+  | [ H : S ?a <= ?b |- context [ ?a <=? ?b ] ] =>
+    rewrite (leb_correct _ _ (le_Sn_le _ _ H))
+  | [ H : ?a < ?b |- context [ ?a <? ?b ] ] =>
+    let X := fresh in
+    assert (a <? b = true) as X by (rewrite Nat.ltb_lt; apply H);
+    rewrite X; clear X
+  | [ |- context [ _ || true ] ] =>
+    rewrite orb_true_r
+  | [ |- context [ true || _ ] ] =>
+    rewrite orb_true_l
+  end.
 
 
 Lemma swap_internal_back tid1 tid2 a1 a2 t:
@@ -1255,19 +1352,23 @@ Proof.
   - inversion T1; chomp1.
   - inversion T1; chomp1.
   - inversion T1; chomp1.
-    all: intros vx I.
-    all: assert (In (tid2, write_item vx) t0) as II by (rewrite H1; now right).
+    all: intros ad' vx I.
+    all: assert (In (tid2, write_item ad' vx) t0) as II by (rewrite H1; now right).
     all: rewrite H1 in II; apply H3 in II; destruct II; [ congruence | assumption ].
   - inversion T1; chomp1.
   - inversion T1; chomp1.
-    all: intros vers' I.
-    all: assert (In (tid2, read_item vers') t0) as II by (rewrite H1; now right).
+    all: intros ad' vers' I.
+    all: assert (In (tid2, read_item ad' vers') t0) as II by (rewrite H1; now right).
     all: rewrite H1 in II; apply H3 in II; destruct II; [ congruence | assumption ].
   - assert (tid2 > 0) by (apply (trace_in_nonzero _ commit_done_txn _ T); now left).
     inversion T1; chomp1.
     all: rewrite <- H6 in *; cbn in H3; try assumption.
-    rewrite H10; omega.
-    all: now rewrite H9.
+    all: intros ad0; destruct (Nat.eq_dec ad ad0).
+    1,3,5: rewrite <- e.
+    rewrite H10; auto.
+    1,2: rewrite H9; auto.
+    all: generalize (H3 ad0).
+    all: destruct (Nat.eq_dec ad0 ad); try congruence.
 Qed.
 
 Lemma swap_internal_forward tid1 tid2 a1 a2 t:
@@ -1292,48 +1393,49 @@ Proof.
 
   - inversion T1; chomp1.
   - rewrite H1 in *; clear H1.
-    replace (write_version ((tid1, a1) :: t)) with (write_version t) in *.
+    replace (write_version ad ((tid1, a1) :: t)) with (write_version ad t) in *.
     inversion T1; check_action; chomp1.
     destruct a1; cbn in Int; try contradiction Int; cbn; reflexivity.
   - inversion T1; chomp1.
   - inversion T1; chomp1.
   - inversion T1; check_action; chomp1.
-    cbn; congruence.
+    intros adx; cbn; destruct (Nat.eq_dec adx ad); congruence.
   - inversion T1; chomp1.
-    all: intros vx I.
-    all: assert (In (tid2, write_item vx) t0) as II by (rewrite H1; now right).
+    all: intros adx vx I.
+    all: assert (In (tid2, write_item adx vx) t0) as II by (rewrite H1; now right).
     all: rewrite H1 in II; apply H3 in II; destruct II; [ congruence | assumption ].
   - inversion T1; check_action; subst; chomp1.
   - inversion T1; chomp1.
   - inversion T1; check_action; chomp1.
     assert (tid1 > 0) as TZ by (apply (trace_in_nonzero _ commit_done_txn _ T1); now left).
-    cbn; omega.
+    intros adx; cbn; destruct (Nat.eq_dec adx ad); auto.
   - inversion T1; chomp1.
-    all: intros vers' I.
-    all: assert (In (tid2, read_item vers') t0) as II by (rewrite H1; now right).
+    all: intros adx vers' I.
+    all: assert (In (tid2, read_item adx vers') t0) as II by (rewrite H1; now right).
     all: rewrite H1 in II; apply H3 in II; destruct II; [ congruence | assumption ].
   - rewrite H1 in *; clear H1.
-    replace (write_version ((tid1, a1) :: t)) with (write_version t) in *.
+    replace (write_version ad ((tid1, a1) :: t)) with (write_version ad t) in *.
     inversion T1; check_action; chomp1.
     assert (tid1 > 0) as TZ by (apply (trace_in_nonzero _ commit_done_txn _ T1); now left).
-    cbn; omega.
+    intros adx; cbn; destruct (Nat.eq_dec adx ad); auto; omega.
     destruct a1; cbn in Int; try contradiction Int; cbn; reflexivity.
   - assert (tid2 > 0) as TZ by (apply (trace_in_nonzero _ commit_done_txn _ T); now left).
     inversion T1; chomp1.
+    all: intros adx.
     all: rewrite <- H5 in *; clear H5.
     all: cbn in H3; try apply H3.
-    rewrite H9; omega.
-    all: now rewrite H8.
+    all: generalize (H3 adx); intros XX.
+    all: destruct (Nat.eq_dec adx ad); auto.
 Qed.
 
-Lemma swap_read_back tid1 tid2 v a1 t:
-  sto_trace ((tid2, read_item v) :: (tid1, a1) :: t) ->
-  action_commute_read a1 ->
+Lemma swap_read_back tid1 tid2 ad v a1 t:
+  sto_trace ((tid2, read_item ad v) :: (tid1, a1) :: t) ->
+  action_commute_read ad a1 ->
   tid1 <> tid2 ->
-  sto_trace ((tid1, a1) :: (tid2, read_item v) :: t).
+  sto_trace ((tid1, a1) :: (tid2, read_item ad v) :: t).
 Proof.
   intros T Int N.
-  assert (tid_phase tid1 ((tid2, read_item v) :: t) = tid_phase tid1 t) as TP1. {
+  assert (tid_phase tid1 ((tid2, read_item ad v) :: t) = tid_phase tid1 t) as TP1. {
     cbn; destruct (Nat.eq_dec tid1 tid2); congruence.
   }
   assert (tid_phase tid2 ((tid1, a1) :: t) = tid_phase tid2 t) as TP2. {
@@ -1341,25 +1443,27 @@ Proof.
   }
 
   inversion T.
-  assert (write_version ((tid1, a1) :: t) = write_version t) as WV. {
-    destruct a1; cbn in Int; try contradiction; cbn; reflexivity.
+  assert (write_version ad ((tid1, a1) :: t) = write_version ad t) as WV. {
+    destruct a1; cbn; auto.
+    destruct (Nat.eq_dec ad ad1); auto.
+    rewrite <- e in Int; cbn in Int; contradiction.
   }
   rewrite WV.
-  rename H4 into T1.
+  rename H5 into T1.
 
   inversion T1; check_action; chomp1.
   all: cbn; destruct (Nat.eq_dec tid1 tid2); [ congruence | auto ].
-  constructor; fix_phase; auto.
+  all: cbn in H4; destruct (Nat.eq_dec ad ad1) as [X|X]; [congruence|auto].
 Qed.
 
-Lemma swap_validate_read_back tid1 tid2 v a1 t:
-  sto_trace ((tid2, validate_read_item v) :: (tid1, a1) :: t) ->
-  action_commute_read a1 ->
+Lemma swap_validate_read_back tid1 tid2 ad v a1 t:
+  sto_trace ((tid2, validate_read_item ad v) :: (tid1, a1) :: t) ->
+  action_commute_read ad a1 ->
   tid1 <> tid2 ->
-  sto_trace ((tid1, a1) :: (tid2, validate_read_item v) :: t).
+  sto_trace ((tid1, a1) :: (tid2, validate_read_item ad v) :: t).
 Proof.
   intros T Int N.
-  assert (tid_phase tid1 ((tid2, validate_read_item v) :: t) = tid_phase tid1 t) as TP1. {
+  assert (tid_phase tid1 ((tid2, validate_read_item ad v) :: t) = tid_phase tid1 t) as TP1. {
     cbn; destruct (Nat.eq_dec tid1 tid2); congruence.
   }
   assert (tid_phase tid2 ((tid1, a1) :: t) = tid_phase tid2 t) as TP2. {
@@ -1367,26 +1471,29 @@ Proof.
   }
 
   inversion T.
-  assert (write_version ((tid1, a1) :: t) = write_version t) as WV. {
-    destruct a1; cbn in Int; try contradiction; cbn; reflexivity.
+  assert (write_version ad ((tid1, a1) :: t) = write_version ad t) as WV. {
+    destruct a1; cbn; auto.
+    destruct (Nat.eq_dec ad ad1); auto.
+    cbn in Int; congruence.
   }
-  rename H7 into T1.
+  rename H8 into T1.
 
   inversion T1; check_action; chomp1.
   all: cbn in WV; auto.
+  all: cbn in H4, H5; destruct (Nat.eq_dec ad ad1) as [X|X]; [congruence|auto].
 Qed.
 
-Lemma swap_read_forward tid1 tid2 v a2 t:
-  sto_trace ((tid2, a2) :: (tid1, read_item v) :: t) ->
-  action_commute_read a2 ->
+Lemma swap_read_forward tid1 tid2 ad v a2 t:
+  sto_trace ((tid2, a2) :: (tid1, read_item ad v) :: t) ->
+  action_commute_read ad a2 ->
   tid1 <> tid2 ->
-  sto_trace ((tid1, read_item v) :: (tid2, a2) :: t).
+  sto_trace ((tid1, read_item ad v) :: (tid2, a2) :: t).
 Proof.
   intros T Int N.
   assert (tid_phase tid1 ((tid2, a2) :: t) = tid_phase tid1 t) as TP1. {
     cbn; destruct (Nat.eq_dec tid1 tid2); congruence.
   }
-  assert (tid_phase tid2 ((tid1, read_item v) :: t) = tid_phase tid2 t) as TP2. {
+  assert (tid_phase tid2 ((tid1, read_item ad v) :: t) = tid_phase tid2 t) as TP2. {
     cbn; destruct (Nat.eq_dec tid2 tid1); congruence.
   }
 
@@ -1395,31 +1502,44 @@ Proof.
        | [ H: sto_trace ((?t1, ?a1) :: ?t), H2: sto_trace (?a :: ?b :: ?c) |- _ ] =>
          rename H into T1
        end.
-  all: inversion T1; chomp1.
-  - cbn; destruct (Nat.eq_dec tid1 tid2); auto.
-  - cbn; fix_phase.
-  - intros vx I.
-    assert (In (tid2, write_item vx) t0) as II by (rewrite H1; now right).
+  all: inversion T1.
+  - chomp1.
+  - chomp1; cbn; auto. now cln. constructor; fix_phase; auto.
+  - chomp1.
+  - chomp1.
+  - chomp1.
+    cbn; destruct (Nat.eq_dec ad ad0); [congruence|auto].
+  - chomp1.
+    intros adx vx I.
+    assert (In (tid2, write_item adx vx) t0) as II by (rewrite H1; now right).
     rewrite H1 in II; apply H3 in II; destruct II; [ congruence | assumption ].
-  - rewrite <- H4; cbn; reflexivity.
-  - intros vers' I.
-    assert (In (tid2, read_item vers') t0) as II by (rewrite H1; now right).
+  - chomp1. cbn in H4; auto.
+  - chomp1.
+  - chomp1.
+    cbn; destruct (Nat.eq_dec ad ad0); [congruence|auto].
+  - chomp1.
+    intros adx vers I.
+    assert (In (tid2, read_item adx vers) t0) as II by (rewrite H1; now right).
     rewrite H1 in II; apply H3 in II; destruct II; [ congruence | assumption ].
-  - assert (tid2 > 0) by (apply (trace_in_nonzero _ commit_done_txn _ T); now left).
-    omega.
+  - cbn.
+    replace (write_version ad t) with (write_version ad ((tid2, complete_write_item ad0 (S (write_version ad0 t))) :: t)).
+    constructor; fix_phase.
+    all: cbn; now cln.
+  - chomp1.
+    intros adx; generalize (H3 adx); intros LL; now cbn in LL.
 Qed.
 
-Lemma swap_validate_read_forward tid1 tid2 v a2 t:
-  sto_trace ((tid2, a2) :: (tid1, validate_read_item v) :: t) ->
-  action_commute_read a2 ->
+Lemma swap_validate_read_forward tid1 tid2 ad v a2 t:
+  sto_trace ((tid2, a2) :: (tid1, validate_read_item ad v) :: t) ->
+  action_commute_read ad a2 ->
   tid1 <> tid2 ->
-  sto_trace ((tid1, validate_read_item v) :: (tid2, a2) :: t).
+  sto_trace ((tid1, validate_read_item ad v) :: (tid2, a2) :: t).
 Proof.
   intros T Int N.
   assert (tid_phase tid1 ((tid2, a2) :: t) = tid_phase tid1 t) as TP1. {
     cbn; destruct (Nat.eq_dec tid1 tid2); congruence.
   }
-  assert (tid_phase tid2 ((tid1, validate_read_item v) :: t) = tid_phase tid2 t) as TP2. {
+  assert (tid_phase tid2 ((tid1, validate_read_item ad v) :: t) = tid_phase tid2 t) as TP2. {
     cbn; destruct (Nat.eq_dec tid2 tid1); congruence.
   }
 
@@ -1431,31 +1551,70 @@ Proof.
   all: inversion T1; chomp1.
   - cbn; destruct (Nat.eq_dec tid1 tid2); [ congruence | auto ].
   - cbn; fix_phase.
-  - intros vx I.
-    assert (In (tid2, write_item vx) t0) as II by (rewrite H1; now right).
+  - cbn; now cln.
+  - intros adx vx I.
+    assert (In (tid2, write_item adx vx) t0) as II by (rewrite H1; now right).
     rewrite H1 in II; apply H3 in II; destruct II; [ congruence | assumption ].
   - rewrite <- H4; cbn; reflexivity.
-  - intros vers' I.
-    assert (In (tid2, read_item vers') t0) as II by (rewrite H1; now right).
+  - cbn; now cln.
+  - intros adx vers' I.
+    assert (In (tid2, read_item adx vers') t0) as II by (rewrite H1; now right).
     rewrite H1 in II; apply H3 in II; destruct II; [ congruence | assumption ].
-  - apply locked_by_self_or in H8.
-    destruct H8.
-    assert (tid2 > 0) by (apply (trace_in_nonzero _ commit_done_txn _ T); now left).
-    omega.
-    rewrite H8; auto.
+  - cbn; now cln.
+  - cbn; now cln.
+  - cbn; now cln.
+  - cbn; apply complete_write_item_step with (val:=val);
+      fix_phase.
+    apply (trace_cons _ _ T1).
+  - intros adx; generalize (H3 adx); intros LL.
+    now cbn in LL.
 Qed.
+
+Definition addresses a ad :=
+  match a with
+  | read_item ad' _
+  | write_item ad' _
+  | lock_write_item ad'
+  | validate_read_item ad' _
+  | unlock_write_item ad'
+  | complete_write_item ad' _ => ad = ad'
+  | _ => False
+  end.
+
+Definition addressof a :=
+  match a with
+  | read_item ad _
+  | write_item ad _
+  | lock_write_item ad
+  | validate_read_item ad _
+  | unlock_write_item ad
+  | complete_write_item ad _ => Some ad
+  | _ => None
+  end.
+
+Definition locked_by_of a t default :=
+  match addressof a with
+  | Some ad => locked_by ad t default
+  | None => default
+  end.
+
+Definition write_version_of a t :=
+  match addressof a with
+  | Some ad => write_version ad t
+  | None => 0
+  end.
 
 Lemma swap_forward_to_seq_point tid1 tid2 a1 a2 t:
   sto_trace ((tid2, a2) :: (tid1, a1) :: t) ->
   tid1 <> tid2 ->
   action_phase a1 < 3 ->
-  locked_by ((tid2, a2) :: t) tid1 = tid1 ->
-  write_version ((tid2, a2) :: t) = write_version t ->
+  locked_by_of a1 ((tid2, a2) :: t) tid1 = tid1 ->
+  write_version_of a1 ((tid2, a2) :: t) = write_version_of a1 t ->
   sto_trace ((tid1, a1) :: (tid2, a2) :: t).
 Proof.
   intros T N AP LB WV.
-  assert (write_version ((tid1, a1) :: t) = write_version t) as WV1. {
-    destruct a1; cbn in AP; try omega.
+  assert (forall ad, write_version ad ((tid1, a1) :: t) = write_version ad t) as WV1. {
+    intros ad; destruct a1; cbn in AP; try omega.
     all: cbn; reflexivity.
   }
   assert (tid1 > 0) as T1Z. {
@@ -1481,39 +1640,55 @@ Proof.
     apply swap_read_back; auto.
     rewrite <- WV1; auto.
     destruct a1; cbn in AP; try omega; cbn; auto.
-    cbn in H3; omega.
-  - cbn in LB; congruence.
+    cbn in H3; destruct (Nat.eq_dec ad ad0); auto; omega.
+  - inversion T1; check_action; chomp1.
+    cbn; cbn in LB; destruct (Nat.eq_dec ad0 ad); [congruence|auto].
+    cbn; cbn in LB; destruct (Nat.eq_dec ad0 ad); [congruence|auto].
+    cbn; cbn in H4; destruct (Nat.eq_dec ad ad0); [congruence|auto].
   - apply swap_validate_read_back; auto.
     destruct a1; cbn in AP; try omega; cbn; auto.
+    cbn in H3; destruct (Nat.eq_dec ad ad0); [congruence|auto].
   - inversion T1; check_action; chomp1.
     all: cbn; auto.
-    cbn in H3; congruence.
-  - cbn in WV; destruct a1; cbn in AP; try omega.
+    1-2: destruct (Nat.eq_dec ad0 ad); auto.
+    cbn in H3; destruct (Nat.eq_dec ad ad0); congruence.
+  - cbn; inversion T1; check_action; chomp1.
+    all: cbn; try now cln.
+    1-2: destruct (Nat.eq_dec ad0 ad); auto.
+    cbn in H3; destruct (Nat.eq_dec ad ad0); [congruence|auto].
 Qed.    
 
-Definition tid_outstanding_read tid (t:trace) :=
-  exists v, In (tid, read_item v) t /\
-            ~ In (tid, validate_read_item v) t.
+Definition tid_outstanding_read tid ad (t:trace) :=
+  exists v, In (tid, read_item ad v) t /\
+            ~ In (tid, validate_read_item ad v) t.
 
-Lemma trace_outstanding_read_head tid v t:
-  sto_trace ((tid, read_item v) :: t) ->
-  tid_outstanding_read tid ((tid, read_item v) :: t).
+Lemma read_outstanding_read tid ad v t:
+  sto_trace ((tid, read_item ad v) :: t) ->
+  tid_outstanding_read tid ad ((tid, read_item ad v) :: t).
 Proof.
   intros T; inversion T.
-  exists (write_version t); split.
+  exists (write_version ad t); split.
   now left.
   intros F; subst.
-  assert (3 <= tid_phase tid ((tid, read_item (write_version t)) :: t)). {
-    replace 3 with (action_phase (validate_read_item (write_version t))) by (now cbn).
+  assert (3 <= tid_phase tid ((tid, read_item ad (write_version ad t)) :: t)). {
+    replace 3 with (action_phase (validate_read_item ad (write_version ad t))) by (now cbn).
     apply phase_increase_in; auto.
   }
   cbn in H; destruct (Nat.eq_dec tid tid); [ omega | congruence ].
 Qed.
 
-Lemma permutation_outstanding_read {tid t1 t2}:
+Lemma validate_outstanding_read tid ad v t:
+  sto_trace ((tid, validate_read_item ad v) :: t) ->
+  tid_outstanding_read tid ad t.
+Proof.
+  intros T; inversion T.
+  exists v; split; auto.
+Qed.
+
+Lemma permutation_outstanding_read {tid ad t1 t2}:
   Permutation t1 t2 ->
-  tid_outstanding_read tid t1 ->
-  tid_outstanding_read tid t2.
+  tid_outstanding_read tid ad t1 ->
+  tid_outstanding_read tid ad t2.
 Proof.
   intros PE H; unfold tid_outstanding_read in *.
   destruct H as [v [I N]].
@@ -1529,24 +1704,24 @@ Inductive trace_unconflicted : trace -> Prop :=
     trace_unconflicted t ->
     action_internal a ->
     trace_unconflicted ((tid, a) :: t)
-| read_unc: forall tid v t,
+| read_unc: forall tid ad v t,
     trace_unconflicted t ->
-    locked_by t 0 = 0 ->
-    write_version t = v ->
-    trace_unconflicted ((tid, read_item v) :: t)
-| validate_read_unc: forall tid v t,
+    locked_by ad t 0 = 0 ->
+    write_version ad t = v ->
+    trace_unconflicted ((tid, read_item ad v) :: t)
+| validate_read_unc: forall tid ad v t,
     trace_unconflicted t ->
-    trace_unconflicted ((tid, validate_read_item v) :: t)
-| lock_unc: forall tid t,
+    trace_unconflicted ((tid, validate_read_item ad v) :: t)
+| lock_unc: forall tid ad t,
     trace_unconflicted t ->
-    (forall tid', tid = tid' \/ ~ tid_outstanding_read tid' t) ->
-    trace_unconflicted ((tid, lock_write_item) :: t)
-| complete_unc: forall tid v t,
+    (forall tid', tid = tid' \/ ~ tid_outstanding_read tid' ad t) ->
+    trace_unconflicted ((tid, lock_write_item ad) :: t)
+| complete_unc: forall tid ad v t,
     trace_unconflicted t ->
-    trace_unconflicted ((tid, complete_write_item v) :: t)
-| unlock_unc: forall tid t,
+    trace_unconflicted ((tid, complete_write_item ad v) :: t)
+| unlock_unc: forall tid ad t,
     trace_unconflicted t ->
-    trace_unconflicted ((tid, unlock_write_item) :: t).
+    trace_unconflicted ((tid, unlock_write_item ad) :: t).
 
 Lemma unconflicted_cons ta t:
   trace_unconflicted (ta :: t) ->
@@ -1580,66 +1755,11 @@ Proof.
 Qed.
 
 
-Lemma phase3_locked tid t:
-  sto_trace t ->
-  tid_phase tid t < 4 ->
-  In (tid, lock_write_item) t ->
-  locked_by t 0 = tid.
-Proof.
-  intros T; induction T; intros P I.
-  all: cbn in *; try contradiction.
-  all: destruct (Nat.eq_dec tid tid0); try omega.
-  all: destruct or I; try congruence; auto.
-  all: assert (2 <= tid_phase tid t) as P2
-      by (replace 2 with (action_phase lock_write_item) by (now cbn);
-          apply phase_increase_in; auto).
-  all: try solve [ rewrite <- e in *; omega ].
-  - rewrite (IHT P I) in H1.
-    assert (tid > 0) by (apply trace_phase_nonzero with (t:=t); auto; omega); omega.
-  - rewrite <- e in *; clear e P.
-    assert (tid_phase tid t < 4) as TL by omega; auto.
-  - rewrite <- e in *; clear e P.
-    assert (tid_phase tid t < 4) as TL by omega; auto.
-  - rewrite (IHT P I) in H0; congruence.
-  - rewrite (IHT P I) in H0; congruence.
-Qed.
-
-Lemma committed_write_locked_or_completed tid t:
+Lemma committed_read_validated tid t ad v:
   sto_trace t ->
   tid_phase tid t = 4 ->
-  In (tid, lock_write_item) t ->
-  locked_by t 0 = tid \/ exists v, In (tid, complete_write_item v) t.
-Proof.
-  intros T; induction T; intros P I.
-  all: cbn in *; try contradiction.
-  all: destruct (Nat.eq_dec tid tid0); try omega.
-  all: destruct or I; try congruence.
-  all: try solve [ generalize (IHT P I); intros X; destruct X as [X | [vv X]];
-                   [ now left | right; exists vv; now right ] ].
-  - generalize (IHT P I); intros X; destruct X as [X | [vv X]].
-    assert (tid > 0) as NZ by (apply trace_phase_nonzero with (t:=t); auto; omega).
-    omega.
-    right; exists vv; now right.
-  - generalize (IHT P I); intros X; destruct X as [X | [vv X]].
-    congruence.
-    right; exists vv; now right.
-  - rewrite <- e in *; clear e P; left.
-    apply phase3_locked; auto; omega.
-  - right; exists (S (write_version t)); rewrite e; now left.
-  - generalize (IHT P I); intros X; destruct X as [X | [vv X]].
-    congruence.
-    right; exists vv; now right.
-  - rewrite <- e in *; clear e P.
-    generalize (IHT H I); intros X; destruct X as [X | [vv X]].
-    now left.
-    right; exists vv; now right.
-Qed.
-
-Lemma committed_read_validated tid t v:
-  sto_trace t ->
-  tid_phase tid t = 4 ->
-  In (tid, read_item v) t ->
-  In (tid, validate_read_item v) t.
+  In (tid, read_item ad v) t ->
+  In (tid, validate_read_item ad v) t.
 Proof.
   intros T; induction T; intros P I.
   all: cbn in *; try contradiction.
@@ -1651,41 +1771,55 @@ Proof.
   - rewrite <- e in *; auto.
 Qed.
 
-Lemma trace_after_lock tid t1 t2:
-  sto_trace (t1 ++ (tid, lock_write_item) :: t2) ->
-  In (tid, unlock_write_item) t1
-  \/ locked_by (t1 ++ (tid, lock_write_item) :: t2) 0 = tid
-  \/ write_version t2 < write_version (t1 ++ (tid, lock_write_item) :: t2).
+Lemma trace_after_lock tid t1 t2 ad:
+  sto_trace (t1 ++ (tid, lock_write_item ad) :: t2) ->
+  In (tid, unlock_write_item ad) t1
+  \/ locked_by ad (t1 ++ (tid, lock_write_item ad) :: t2) 0 = tid
+  \/ write_version ad t2 < write_version ad (t1 ++ (tid, lock_write_item ad) :: t2).
 Proof.
   induction t1; intros T.
-  right; left; now cbn.
+  right; left; cbn; now cln.
   destruct a; inversion T; rewrite <- H0 in *; clear H0.
   all: match goal with
        | [ H: sto_trace (_ ++ _ :: _) |- _ ] =>
          rename H into T1; generalize (IHt1 T1); intros X
        end.
-  all: destruct X as [X | [X | X]]; intuition.
-  - assert (tid > 0). {
-      apply (trace_in_nonzero _ lock_write_item _ T1).
-      apply in_or_app; right; now left.
-    }
-    omega.
-  - rewrite H3 in X; rewrite X; left; now left.
-  - rewrite H3 in X; rewrite X in *; clear X t.
-    cbn; right; right.
+  all: destruct X as [X|[X|X]]; intuition.
+  - right; left; cbn.
+    destruct (Nat.eq_dec ad ad0); auto.
+    rewrite <- e in *; clear e; rewrite H4 in H0.
+    enough (tid > 0); [omega|].
+    apply (trace_in_nonzero _ (lock_write_item ad) _ T1).
+    apply in_or_app; right; now left.
+  - destruct (Nat.eq_dec ad ad0).
+    rewrite <- e in *; clear e; left; left.
+    rewrite <- H0; now rewrite H3.
+    right; left; cbn; now cln.
+  - cbn; destruct (Nat.eq_dec ad ad0); [rewrite <- e in *; clear e|].
+    right; right.
     apply le_lt_n_Sm.
-    apply write_version_increase_app in T1; now cbn in T1.
-  - cbn; right; right; omega.
-  - cbn; right; right; omega.
-  - cbn; right; right; omega.
+    replace ((tid, lock_write_item ad) :: t2)
+    with ([(tid, lock_write_item ad)] ++ t2) by (now cbn).
+    rewrite app_assoc.
+    apply write_version_increase_app.
+    rewrite <- app_assoc; cbn.
+    rewrite <- app_comm_cons in *.
+    now apply trace_cons in T.
+    right; now left.
+  - cbn; destruct (Nat.eq_dec ad ad0);
+      [right; right; rewrite <- e; auto | right; now left].
+  - cbn; destruct (Nat.eq_dec ad ad0);
+      [right; right; rewrite <- e; auto | right; now left].
+  - cbn; destruct (Nat.eq_dec ad ad0);
+      [right; right; rewrite <- e; auto | right; now right].
 Qed.
   
-Lemma nonaborted_read_validate_different tid tid' t1 t2 v:
-  sto_trace (t1 ++ (tid, lock_write_item) :: t2) ->
-  tid_phase tid (t1 ++ (tid, lock_write_item) :: t2) < 6 ->
+Lemma nonaborted_read_validate_different tid tid' t1 t2 ad v:
+  sto_trace (t1 ++ (tid, lock_write_item ad) :: t2) ->
+  tid_phase tid (t1 ++ (tid, lock_write_item ad) :: t2) < 6 ->
   tid <> tid' ->
-  In (tid', read_item v) t2 ->
-  ~ In (tid', validate_read_item v) t1.
+  In (tid', read_item ad v) t2 ->
+  ~ In (tid', validate_read_item ad v) t1.
 Proof.
   induction t1; intros T P N I.
   intros F; destruct F.
@@ -1706,22 +1840,21 @@ Proof.
   all: destruct F as [F | F]; [ try congruence | ].
   all: try solve [revert F; apply IHt1; auto; try omega].
   rename H7 into T1.
-  generalize (trace_after_lock _ _ _ T1); intros X.
+  generalize (trace_after_lock _ _ _ _ T1); intros X.
   destruct X as [X | [X | X]].
-  - assert (6 <= tid_phase tid (t1 ++ (tid, lock_write_item) :: t2)). {
-      replace 6 with (action_phase unlock_write_item) by (now cbn).
+  - assert (6 <= tid_phase tid (t1 ++ (tid, lock_write_item ad) :: t2)). {
+      replace 6 with (action_phase (unlock_write_item ad)) by (now cbn).
       apply phase_increase_in; auto.
       apply in_or_app; now left.
     }
     omega.
   - apply (locked_by_other tid0) in X; auto.
     congruence.
-    apply (trace_in_nonzero _ lock_write_item _ T1).
+    apply (trace_in_nonzero _ (lock_write_item ad) _ T1).
     apply in_or_app; right; now left.
-  - rewrite H4 in *; clear H4.
-    inversion F; clear F.
+  - inversion F; rewrite <- H7, H8 in *; clear H7 H8 F.
     rewrite H4 in *; clear vers H4.
-    assert (v <= write_version t2). {
+    assert (v <= write_version ad0 t2). {
       apply read_version_increase_in with (tid0:=tid').
       apply trace_app in T1; now apply trace_cons in T1.
       auto.
@@ -1745,21 +1878,21 @@ Proof.
   all: try solve [apply internal_unc; [| cbn]; auto; myexists].
   - apply read_unc; auto; myexists.
   - apply lock_unc; [ myexists | ].
-    remember (t2 ++ (tid0, lock_write_item) :: t) as tb.
+    remember (t2 ++ (tid0, lock_write_item ad) :: t) as tb.
     intros tid; destruct (Nat.eq_dec tid0 tid); [ now left | right ].
     intros F; destruct F as [vers [ER ENV]].
     assert (tid_phase tid tb = 4) as TP4X. {
       apply NU2.
-      assert (In (tid, read_item vers) tb) as EX. {
+      assert (In (tid, read_item ad vers) tb) as EX. {
         rewrite Heqtb; apply in_or_app; right; now right.
       }
       apply phase_increase_in in EX; cbn in EX; auto; omega.
     }
-    assert (In (tid, read_item vers) tb) as ERX. {
+    assert (In (tid, read_item ad vers) tb) as ERX. {
       rewrite Heqtb; apply in_or_app; right; now right.
     }
-    generalize (committed_read_validated _ _ _ NU1 TP4X ERX); intros EVXB.
-    assert (In (tid, validate_read_item vers) t2) as EVX. {
+    generalize (committed_read_validated _ _ _ _ NU1 TP4X ERX); intros EVXB.
+    assert (In (tid, validate_read_item ad vers) t2) as EVX. {
       rewrite Heqtb in EVXB; apply in_app_or in EVXB.
       destruct or EVXB; auto.
       destruct EVXB; [ congruence | contradiction ].
@@ -1770,7 +1903,7 @@ Proof.
     contradiction.
     assert (tid_phase tid0 tb = 4) as TP4. {
       apply NU2.
-      assert (In (tid0, lock_write_item) tb) as EX. {
+      assert (In (tid0, lock_write_item ad) tb) as EX. {
         rewrite Heqtb; apply in_or_app; right; now left.
       }
       apply phase_increase_in in EX; cbn in EX.
@@ -1813,53 +1946,80 @@ Proof.
 
   1, 3, 4: apply swap_internal_forward; cbn; auto.
 
-  - replace (write_version t) with (write_version ((tid2, a2) :: t)).
+  - replace (write_version ad t) with (write_version ad ((tid2, a2) :: t)).
     constructor.
     now rewrite TP1.
-    destruct a2; cbn; auto.
-    inversion U.
-    simpl in H9; contradiction.
-    generalize (H8 tid1); intros X; destruct X as [X | X].
-    congruence.
-    contradict X.
-    apply trace_outstanding_read_head; auto.
+    {
+      destruct a2; cbn; auto.
+      inversion U.
+      check_action.
+      destruct (Nat.eq_dec ad ad1); [rewrite <- e in *; clear e|]; auto.
+      generalize (H10 tid1); intros X; destruct X as [X | X].
+      congruence.
+      contradict X.
+      apply read_outstanding_read; auto.
 
-    destruct a2; inversion T.
-    all: try constructor; fix_phase; auto.
-    cbn; constructor; fix_phase; auto.
-    intros vv I.
-    assert (In (tid2, write_item vv) ((tid1, read_item v) :: t)) as II by (now right).
-    apply (H8 vv) in II; destruct II; [ congruence | assumption ].
-    intros vers I.
-    assert (In (tid2, read_item vers) ((tid1, read_item v) :: t)) as II by (now right).
-    apply (H8 vers) in II; destruct II; [ congruence | assumption ].
-    rewrite H7, H1 in *; clear H7 H1.
-    cbn in *.
-    apply complete_write_item_step with (val:=val); fix_phase; auto.
-    destruct (Nat.eq_dec tid2 tid1); [ congruence | assumption ].
-    destruct (Nat.eq_dec tid2 tid1); assumption.
-
-    destruct a2; cbn; auto.
-    inversion T.
-    simpl in H9; omega.
+      destruct (Nat.eq_dec ad ad1); auto.
+      destruct (Nat.eq_dec ad ad1); auto.
+    }
+    {
+      destruct a2; inversion T.
+      all: try constructor; fix_phase; auto.
+      cbn; constructor; fix_phase; auto.
+      intros adx vv I.
+      assert (In (tid2, write_item adx vv) ((tid1, read_item ad vers) :: t)) as II by (now right).
+      apply (H9 adx vv) in II; destruct II; [ congruence | assumption ].
+      intros adx vers' I.
+      assert (In (tid2, read_item adx vers') ((tid1, read_item ad vers) :: t)) as II by (now right).
+      apply (H9 adx vers') in II; destruct II; [ congruence | assumption ].
+      rewrite H9 in *; clear H9.
+      cbn in *.
+      apply complete_write_item_step with (val:=val); fix_phase; auto.
+      destruct (Nat.eq_dec tid2 tid1); [ congruence | assumption ].
+      destruct (Nat.eq_dec tid2 tid1); assumption.
+    }
+    {
+      destruct a2; cbn; auto.
+      inversion T.
+      destruct (Nat.eq_dec ad ad1); auto.
+      rewrite <- e in *; clear e.
+      inversion H13.
+      cbn in H11; rewrite H11 in H19; omega.
+    }
 
   - apply lock_write_item_step with (v:=v).
     now rewrite TP1.
     now right.
     cbn; destruct a2; auto.
-    inversion T; simpl in H9.
+    destruct (Nat.eq_dec ad ad1); auto.
+    rewrite <- e in *; clear e.
+    inversion T; simpl in H11; cln.
     omega.
+    destruct (Nat.eq_dec ad ad1); auto.
+    destruct (Nat.eq_dec ad ad1); auto.
     destruct a2; inversion T.
     all: try solve [ cbn in *; contradiction ].
     all: try constructor; fix_phase; auto.
-    cbn in H9; rewrite H9 in *; omega.
-    intros vv I.
-    assert (In (tid2, write_item vv) ((tid1, lock_write_item) :: t)) as II by (now right).
-    apply (H8 vv) in II; destruct II; [ congruence | assumption ].
-    intros vers I.
-    assert (In (tid2, read_item vers) ((tid1, lock_write_item) :: t)) as II by (now right).
-    apply (H8 vers) in II; destruct II; [ congruence | assumption ].
-    omega.
+    cbn; constructor; cbn in H9; cln; auto.
+    cbn in H11; destruct (Nat.eq_dec ad1 ad); [omega|auto].
+    cbn in H11; destruct (Nat.eq_dec ad1 ad); [omega|auto].
+    intros adx vv I.
+    assert (In (tid2, write_item adx vv) ((tid1, lock_write_item ad) :: t)) as II by (now right).
+    apply (H9 adx vv) in II; destruct II; [ congruence | assumption ].
+    cbn in H11; destruct (Nat.eq_dec ad1 ad); [congruence|auto].
+    cbn in H10; destruct (Nat.eq_dec ad1 ad); [congruence|auto].
+    intros adx vers I.
+    assert (In (tid2, read_item adx vers) ((tid1, lock_write_item ad) :: t)) as II by (now right).
+    apply (H9 adx vers) in II; destruct II; [ congruence | assumption ].
+    cbn; apply complete_write_item_step with (val:=val); auto.
+    fix_phase.
+    cbn in H11; destruct (Nat.eq_dec ad1 ad); [congruence|auto].
+    cbn in H12; destruct (Nat.eq_dec tid2 tid1); auto.
+    intros adx.
+    enough (locked_by adx ((tid1, lock_write_item ad) :: t) 0 <> tid2).
+    cbn in H12; destruct (Nat.eq_dec adx ad); auto.
+    rewrite e; rewrite H4; omega.
+    apply H9.
 Qed.
 
 Lemma swap_backward_committing tid1 tid2 a1 a2 t:
@@ -1909,21 +2069,70 @@ Proof.
       apply locked_by_self_or in L1; destruct or L1; congruence || omega || idtac
     end.
 
-  - chomp2.
-  - chomp2.
-  - cbn in H11.
-    try rewrite H, H0, H8 in *; clear H H0 H8 vers0 tid3 t1.
-    rewrite <- H11 in *; rewrite H4 in *; clear H11 v.
-    assert (write_version ((tid2, validate_read_item vers) :: t) = vers) as WV2 by (cbn; now rewrite H4).
-    rewrite <- WV2 at 1; constructor; try rewrite WV2; fix_phase; auto.
-  - chomp2.
+  - apply lock_write_item_step with (v:=v); fix_phase.
+    cbn in H9; destruct (Nat.eq_dec ad0 ad); [congruence|auto].
+    now cbn in H10.
+  - apply lock_write_item_step with (v:=v); cbn; fix_phase.
+    destruct (Nat.eq_dec tid1 tid2); [congruence|auto].
+    now right.
+    destruct (Nat.eq_dec ad ad0); auto.
+    cbn in H9; destruct (Nat.eq_dec ad0 ad); [congruence|auto].
+  - constructor; cbn in *; fix_phase; auto.
+    destruct (Nat.eq_dec tid1 tid2); destruct (Nat.eq_dec tid2 tid1); try congruence; auto.
+    inversion T1.
+    contradict H14.
+    destruct H14; [now left|contradiction].
+    destruct (Nat.eq_dec tid2 tid1); [congruence|auto].
+    destruct H13; [congruence|auto].
+  - cbn in *; constructor; fix_phase; cln; auto.
+    cbn; destruct (Nat.eq_dec tid1 tid2); [congruence|auto].
+    destruct (Nat.eq_dec tid2 tid1); [omega|].
+    cbn; destruct (Nat.eq_dec ad ad0); auto.
+    cbn; destruct (Nat.eq_dec ad ad0); auto.
+    rewrite <- e in *; clear e.
+    apply locked_by_self_or in H3; destruct H3; rewrite H1 in *; [omega|congruence].
+    apply complete_write_item_step with (val:=val); auto.
+    cln; auto.
+    now destruct (Nat.eq_dec tid2 tid1).
+  - replace (write_version ad t) with (write_version ad ((tid2, seq_point) :: t)).
+    apply complete_write_item_step with (val:=val); cbn; fix_phase; auto.
+    now cln.
+    now cln.
+    intros adx vx I.
+    enough (In (tid2, lock_write_item adx) ((tid1, complete_write_item ad (S (write_version ad t))) :: t)).
+    destruct H1; [congruence|auto].
+    apply (H7 adx vx); now right.
+    now cbn.
+  - assert (ad0 <> ad) as AD. {
+      destruct (Nat.eq_dec ad0 ad); [|auto].
+      rewrite e in *; clear e.
+      cbn in H10; cln; rewrite H10 in *.
+      cbn in H11; destruct H11; [congruence|].
+      apply read_version_increase_in in H1.
+      rewrite <- H10 in H1; omega.
+      apply (trace_cons _ _ H13).
+    }
+    replace (write_version ad t) with (write_version ad ((tid2, validate_read_item ad0 vers) :: t)).
+    apply complete_write_item_step with (val:=val); cbn; fix_phase; auto.
+    now cln.
+    now cln.
+    cbn in H9; destruct (Nat.eq_dec ad0 ad); [congruence|auto].
+    cbn in H10; destruct (Nat.eq_dec ad0 ad); [congruence|auto].
+    now cbn.
   - apply swap_internal_back; cbn; auto.
-  - cbn in H9.
-    destruct H10; [ congruence | ].
-    apply read_version_increase_in in H1; auto.
-    rewrite <- H9 in H1; omega.
-  - apply swap_internal_back; cbn; auto.
-  - chomp2; omega.
+  - assert (ad0 <> ad) as AD. {
+      destruct (Nat.eq_dec ad0 ad); [|auto].
+      rewrite e, H7 in *; clear e H7.
+      cbn in H9; cln; omega.
+    }
+    cbn; cln.
+    replace (write_version ad t) with (write_version ad ((tid2, complete_write_item ad0 (S (write_version ad0 t))) :: t)).
+    apply complete_write_item_step with (val:=val); cbn; fix_phase; auto.
+    now cln.
+    now cln.
+    now cln.
+    cbn in H9; now cln.
+    cbn; now cln.
   - apply swap_internal_back; cbn; auto.
 Qed.
 
@@ -1978,9 +2187,9 @@ Qed.
 
 Definition trace_same_end_state t1 t2 :=
   Permutation t1 t2
-  /\ locked_by t1 0 = locked_by t2 0
-  /\ write_version t1 = write_version t2
-  /\ forall tid, trace_tid_last_write tid t1 = trace_tid_last_write tid t2.
+  /\ (forall ad, locked_by ad t1 0 = locked_by ad t2 0)
+  /\ (forall ad, write_version ad t1 = write_version ad t2)
+  /\ (forall tid ad, tid_last_write tid ad t1 = tid_last_write tid ad t2).
 
 Lemma trace_same_end_state_cons t1 t2 a:
   trace_same_end_state t1 t2 ->
@@ -1988,11 +2197,14 @@ Lemma trace_same_end_state_cons t1 t2 a:
 Proof.
   intros S; destruct S as [P [L [WV LW]]].
   split; [ | split; [ | split ]].
-  now apply perm_skip.
-  destruct a; destruct a; now cbn.
-  destruct a; destruct a; now cbn.
-  intros tid; destruct a; destruct a; cbn.
-  all: destruct (Nat.eq_dec tid t); auto.
+  - now apply perm_skip.
+  - intros ad; destruct a; destruct a; cbn; auto.
+    all: destruct (Nat.eq_dec ad ad0); auto.
+  - intros ad; destruct a; destruct a; cbn; auto.
+    all: destruct (Nat.eq_dec ad ad0); auto.
+  - intros tid ad; destruct a; destruct a; cbn; auto.
+    all: destruct (Nat.eq_dec tid t); auto.
+    all: destruct (Nat.eq_dec ad ad0); auto.
 Qed.
 
 Lemma trace_same_end_state_app t1 t2 th:
@@ -2028,9 +2240,9 @@ Proof.
     apply Permutation_in with (l:=t1); auto.
     now rewrite <- L.
   - constructor; try rewrite <- PE; auto.
-    intros vv I.
+    intros ad vv I.
     apply Permutation_in with (l:=t1); auto.
-    apply (H3 vv).
+    apply (H3 ad vv).
     apply Permutation_in with (l:=t2); auto.
   - constructor; try rewrite <- PE; auto.
     apply locked_by_self_or in H3.
@@ -2045,7 +2257,7 @@ Proof.
   - constructor; try rewrite <- PE; auto.
     now rewrite <- L.
   - constructor; try rewrite <- PE; auto.
-    intros vv I.
+    intros ad vv I.
     apply Permutation_in with (l:=t1); auto.
     apply H3.
     apply Permutation_in with (l:=t2); auto.
@@ -2054,7 +2266,7 @@ Proof.
     now rewrite <- L.
     now rewrite <- LW.
   - constructor; try rewrite <- PE; auto.
-    now rewrite <- L.
+    intros ad; now rewrite <- L.
     contradict H4.
     apply Permutation_in with (l:=t2); auto.
 Qed.
@@ -2121,12 +2333,19 @@ Proof.
   }
   split; [ | split; [ | split ]].
   - constructor.
-  - cbn; destruct a1; destruct a2; try congruence.
-    all: inversion T; cbn in *; try congruence; omega.
-  - cbn; destruct a1; destruct a2; try congruence.
-    all: inversion T; cbn in *; try congruence; omega.
-  - intros tid; cbn.
-    destruct (Nat.eq_dec tid tid1); destruct (Nat.eq_dec tid tid2);
+  - intros adx.
+    cbn; destruct a1; check_action; destruct a2; try congruence.
+    all: inversion T; cbn in *; try congruence.
+    all: destruct (Nat.eq_dec adx ad0); destruct (Nat.eq_dec adx ad); auto.
+    all: subst; repeat cln; omega.
+  - intros adx.
+    cbn; destruct a1; check_action; destruct a2; try congruence.
+    all: inversion T; cbn in *; try congruence.
+    all: destruct (Nat.eq_dec adx ad0); destruct (Nat.eq_dec ad0 ad); auto.
+    all: subst; repeat cln; omega.
+  - intros tid adx.
+    cbn; destruct a1; check_action; destruct a2; try congruence.
+    all: destruct (Nat.eq_dec tid tid1); destruct (Nat.eq_dec tid tid2);
       congruence.
 Qed.
 
@@ -2153,12 +2372,19 @@ Proof.
   }
   split; [ | split; [ | split ]].
   - constructor.
-  - cbn; destruct a1; destruct a2; try congruence.
-    all: inversion T; cbn in *; try congruence; omega.
-  - cbn; destruct a1; destruct a2; try congruence.
-    all: inversion T; cbn in *; try congruence; omega.
-  - intros tid; cbn.
-    destruct (Nat.eq_dec tid tid1); destruct (Nat.eq_dec tid tid2);
+  - intros adx.
+    cbn; destruct a2; check_action; destruct a1; try congruence.
+    all: inversion T; cbn in *; try congruence.
+    all: destruct (Nat.eq_dec adx ad); destruct (Nat.eq_dec adx ad0); auto.
+    all: subst; repeat cln; omega.
+  - intros adx.
+    cbn; destruct a2; check_action; destruct a1; try congruence.
+    all: inversion T; cbn in *; try congruence.
+    all: destruct (Nat.eq_dec adx ad); destruct (Nat.eq_dec adx ad0); auto.
+    all: subst; repeat cln; omega.
+  - intros tid adx.
+    cbn; destruct a2; check_action; destruct a1; try congruence.
+    all: destruct (Nat.eq_dec tid tid1); destruct (Nat.eq_dec tid tid2);
       congruence.
 Qed.
 
@@ -2192,10 +2418,9 @@ Proof.
     inversion U.
     - now apply internal_unc.
     - apply read_unc; auto.
-      + destruct a1; cbn in H3; auto.
-        all: cbn in AP; omega.
-      + destruct a1; cbn in H4; auto.
-        cbn in AP; omega.
+      + destruct a1; cbn in H3; check_action; auto.
+        destruct (Nat.eq_dec ad ad0); [omega|auto].
+      + destruct a1; cbn in H4; check_action; auto.
     - apply validate_read_unc; auto.
     - apply lock_unc; auto.
       intros tid'.
@@ -2215,32 +2440,36 @@ Proof.
   - now apply internal_unc.
   - apply read_unc; auto.
     + destruct a2; cbn; auto.
+      all: destruct (Nat.eq_dec ad ad0); auto.
+      rewrite <- e in *; clear e.
       subst.
       inversion U; [ cbn in *; contradiction | ].
-      generalize (H4 tid1); intros X; destruct X.
+      generalize (H5 tid1); intros X; destruct X.
       congruence.
-      contradict H5.
-      exists (write_version t).
+      contradict H6.
+      exists (write_version ad t).
       split; [ now left | ].
-      intros I; destruct I.
-      inversion H5.
-      apply phase_increase_in in H5; simpl in H5; auto.
+      intros I; destruct I as [I|I].
+      inversion I.
+      apply phase_increase_in in I; simpl in I; auto.
       apply trace_cons in T; apply phase_increase_head in T; omega.
       do 2 apply trace_cons in T; auto.
     + destruct a2; cbn; auto.
-      rewrite <- H0 in *.
-      inversion T; simpl in H9; omega.
+      destruct (Nat.eq_dec ad ad0); auto.
+      rewrite <- H0 in *; clear a1 H0.
+      rewrite <- e in *; clear ad0 e.
+      inversion T.
+      cbn in H9; rewrite H3 in H9; omega.
   - apply validate_read_unc; auto.
   - apply lock_unc; auto.
     intros t'; generalize (H3 t'); intros X; destruct X.
     now left.
     right; contradict H4.
     destruct H4 as [V [I NI]]; exists V; split.
-    destruct I.
-    inversion H4; subst.
+    destruct I as [I|I]; auto.
+    inversion I; subst.
     inversion U; [cbn in *; contradiction|].
-    simpl in H6; omega.
-    auto.
+    simpl in H6; cln; omega.
     contradict NI; now right.
   - apply complete_unc; auto.
   - apply unlock_unc; auto.
@@ -2276,10 +2505,8 @@ Proof.
     inversion U; subst.
     - now apply internal_unc.
     - apply read_unc; auto.
-      + destruct a1; cbn in H3; auto.
-        all: cbn in AP; omega.
-      + destruct a1; cbn in H3; auto.
-        cbn in AP; omega.
+      + destruct a1; check_action; auto.
+      + destruct a1; check_action; auto.
     - apply validate_read_unc; auto.
     - apply lock_unc; auto.
       intros tid'.
@@ -2290,29 +2517,19 @@ Proof.
       exists V; split.
       now right.
       contradict NI.
-      destruct NI; auto.
-      inversion H; subst; cbn in AP; omega.
+      destruct NI as [NI|NI]; auto.
+      inversion NI; subst; cbn in AP; omega.
     - apply complete_unc; auto.
     - apply unlock_unc; auto.
   }
   inversion U1.
   - now apply internal_unc.
   - apply read_unc; auto.
-    + destruct a2; cbn; auto.
-      subst.
-      inversion U; [ cbn in *; contradiction | ].
-      generalize (H4 tid1); intros X; destruct X.
-      congruence.
-      contradict H5.
-      exists (write_version t).
-      split; [ now left | ].
-      intros I; destruct I.
-      inversion H5.
-      apply phase_increase_in in H5; simpl in H5; auto.
-      apply trace_cons in T; apply phase_increase_head in T; cbn in T; omega.
-      do 2 apply trace_cons in T; auto.
-    + destruct a2; cbn; auto.
-      rewrite <- H0 in *.
+    + destruct a2; check_action; auto.
+      all: cbn; destruct (Nat.eq_dec ad ad0); auto.
+    + destruct a2; check_action; auto.
+      all: cbn; destruct (Nat.eq_dec ad ad0); auto.
+      rewrite <- H0 in *; rewrite <- e in *; clear a1 H0 ad0 e.
       inversion T; simpl in H9; omega.
   - apply validate_read_unc; auto.
   - apply lock_unc; auto.
@@ -2320,11 +2537,10 @@ Proof.
     now left.
     right; contradict H4.
     destruct H4 as [V [I NI]]; exists V; split.
-    destruct I.
-    inversion H4; subst.
+    destruct I as [I|I]; auto.
+    inversion I; subst.
     inversion U; [cbn in *; contradiction|].
-    simpl in H6; omega.
-    auto.
+    simpl in H6; cln; omega.
     contradict NI; now right.
   - apply complete_unc; auto.
   - apply unlock_unc; auto.
@@ -2420,47 +2636,71 @@ Qed.
 
 
 Definition example_txn:=
-  [(2, commit_done_txn); (2, complete_write_item 1); (2, commit_txn);
-     (2, validate_read_item 0); (2, seq_point); (2, lock_write_item);
-       (2, try_commit_txn); (2, write_item 4); (2, read_item 0);
-         (2, start_txn);
-   (1, commit_done_txn); (1, commit_txn); (1, validate_read_item 0);
-     (1, seq_point); (1, try_commit_txn); (1, read_item 0); (1, start_txn)].
+  [ (2, commit_done_txn);
+      (2, complete_write_item 0 1);
+      (2, commit_txn);
+      (2, validate_read_item 0 0);
+      (2, seq_point);
+      (2, lock_write_item 0);
+      (2, try_commit_txn);
+      (2, write_item 0 4);
+      (2, read_item 0 0);
+      (2, start_txn);
+      (1, commit_done_txn);
+      (1, commit_txn);
+      (1, validate_read_item 0 0);
+      (1, seq_point);
+      (1, try_commit_txn);
+      (1, read_item 0 0);
+      (1, start_txn)].
 
 Definition example_txn2:=
-  [(3, commit_done_txn); (3, commit_txn); (3, validate_read_item 1);
-     (3, seq_point); (3, try_commit_txn); (3, read_item 1); (3, start_txn);
-   (1, abort_txn); (1, validate_read_item 1); (1, try_commit_txn);
-   (2, commit_txn); (2, complete_write_item 1); (2, commit_txn);
-     (2, validate_read_item 0); (2, seq_point); (2, lock_write_item);
-       (2, try_commit_txn); (2, write_item 4);
-   (1, read_item 0);
-   (2, read_item 0); (2, start_txn);
-   (1, start_txn)].
+  [ (3, commit_done_txn);
+      (3, commit_txn);
+      (3, validate_read_item 0 1);
+      (3, seq_point);
+      (3, try_commit_txn);
+      (3, read_item 0 1);
+      (3, start_txn);
+      (1, abort_txn);
+      (1, validate_read_item 0 1);
+      (1, try_commit_txn);
+      (2, commit_txn);
+      (2, complete_write_item 0 1);
+      (2, commit_txn);
+      (2, validate_read_item 0 0);
+      (2, seq_point);
+      (2, lock_write_item 0);
+      (2, try_commit_txn);
+      (2, write_item 0 4);
+      (1, read_item 0 0);
+      (2, read_item 0 0);
+      (2, start_txn);
+      (1, start_txn)].
 
 
 Definition example_txn3 :=
   [  (3, commit_done_txn);
      (3, commit_txn);
-     (3, validate_read_item 2);
+     (3, validate_read_item 0 2);
      (3, seq_point);
      (3, try_commit_txn);
-     (3, read_item 2);
+     (3, read_item 0 2);
      (2, commit_done_txn);
-     (2, complete_write_item 2);
+     (2, complete_write_item 0 2);
      (2, commit_txn);
      (3, start_txn);
      (1, commit_done_txn);
      (2, seq_point);
-     (2, lock_write_item);
-     (1, complete_write_item 1);
+     (2, lock_write_item 0);
+     (1, complete_write_item 0 1);
      (1, commit_txn);
      (1, seq_point);
-     (1, lock_write_item);
+     (1, lock_write_item 0);
      (2, try_commit_txn);
-     (2, write_item 0);
+     (2, write_item 0 0);
      (1, try_commit_txn);
-     (1, write_item 1);
+     (1, write_item 0 1);
      (1, start_txn);
      (2, start_txn) ].
 
@@ -2540,13 +2780,27 @@ Qed.
 
 Lemma swap_permutation_last_write {t1 t2}:
   swap_permutation t1 t2 ->
-  forall tid, trace_tid_last_write tid t1 = trace_tid_last_write tid t2.
+  forall tid ad, tid_last_write tid ad t1 = tid_last_write tid ad t2.
 Proof.
   intros SP; induction SP; intros tid; auto.
-  - destruct x; cbn; destruct (Nat.eq_dec tid t); destruct a; auto.
+  - intros ad; destruct x; cbn; destruct (Nat.eq_dec tid t); destruct a; auto.
+    all: destruct (Nat.eq_dec ad ad0); auto.
   - apply swappable_iff in H; destruct H as [I1 [I2 I3]].
     cbn; destruct (Nat.eq_dec tid tid2); destruct (Nat.eq_dec tid tid1); congruence.
   - congruence.
+Qed.
+
+Lemma swap_permutation_refl_skip x t:
+  (forall t2, swap_permutation (x :: t) t2 -> x :: t = t2) ->
+  forall t2, swap_permutation t t2 -> t = t2.
+Proof.
+  intros.
+  assert (x :: t = x :: t2 -> t = t2). {
+    intros; inversion H1; auto.
+  }
+  apply H1.
+  apply H.
+  now constructor.
 Qed.
 
 Lemma swap_permutation_trace t1 t2:
@@ -2556,8 +2810,8 @@ Lemma swap_permutation_trace t1 t2:
   no_aborted t1 ->
     sto_trace t2
     /\ trace_unconflicted t2
-    /\ locked_by t1 0 = locked_by t2 0
-    /\ write_version t1 = write_version t2.
+    /\ (forall ad, locked_by ad t1 0 = locked_by ad t2 0)
+    /\ (forall ad, write_version ad t1 = write_version ad t2).
 Proof.
   intros SP T U NA; induction SP; auto.
   - generalize (trace_cons _ _ T); intros T1.
@@ -2572,8 +2826,8 @@ Proof.
     destruct x; split; [| split; [| split]].
     apply sto_trace_permutation_cons with (t1:=t1); auto.
     apply unconflicted_permutation_cons with (t1:=t1); auto.
-    simpl; repeat rewrite L; auto.
-    simpl; repeat rewrite WV; auto.
+    intros ad; simpl; repeat rewrite L; auto.
+    intros ad; simpl; repeat rewrite WV; auto.
 
   - rewrite swappable_iff in H.
     destruct H as [SS [ST SA]].
@@ -2634,19 +2888,6 @@ Proof.
   intros; apply serial_cons in H; auto.
 Qed.
 
-Lemma swap_permutation_refl_skip x t:
-  (forall t2, swap_permutation (x :: t) t2 -> x :: t = t2) ->
-  forall t2, swap_permutation t t2 -> t = t2.
-Proof.
-  intros.
-  assert (x :: t = x :: t2 -> t = t2). {
-    intros; inversion H1; auto.
-  }
-  apply H1.
-  apply H.
-  now constructor.
-Qed.
-
 
 Lemma rev_split {A:Type} (l:list A):
   l = [] \/ exists l1 a, l = l1 ++ [a].
@@ -2655,40 +2896,6 @@ Proof.
   now left.
   right; now exists l, x.
 Qed.
-
-Ltac cln :=
-  match goal with
-  | [ |- context [ Nat.eq_dec ?a ?a ] ] =>
-    let X := fresh in
-    destruct (Nat.eq_dec a a) as [X|X]; [ | congruence ]; clear X
-  | [ H : context [ Nat.eq_dec ?a ?a ] |- _ ] =>
-    let X := fresh in
-    destruct (Nat.eq_dec a a) as [X|X]; [ | congruence ]; clear X
-  | [ H : ?a = ?b |- context [ Nat.eq_dec ?a ?b ] ] =>
-    let X := fresh in
-    destruct (Nat.eq_dec a b) as [X|X]; [ | congruence ]; clear X
-  | [ H : ?a <> ?b |- context [ Nat.eq_dec ?a ?b ] ] =>
-    let X := fresh in
-    destruct (Nat.eq_dec a b) as [X|X]; [ congruence | ]; clear X
-  | [ H : ?a = ?b |- context [ Nat.eq_dec ?b ?a ] ] =>
-    let X := fresh in
-    destruct (Nat.eq_dec b a) as [X|X]; [ | congruence ]; clear X
-  | [ H : ?a <> ?b |- context [ Nat.eq_dec ?b ?a ] ] =>
-    let X := fresh in
-    destruct (Nat.eq_dec b a) as [X|X]; [ congruence | ]; clear X
-  | [ H : ?a <= ?b |- context [ ?a <=? ?b ] ] =>
-    rewrite (leb_correct _ _ H)
-  | [ H : S ?a <= ?b |- context [ ?a <=? ?b ] ] =>
-    rewrite (leb_correct _ _ (le_Sn_le _ _ H))
-  | [ H : ?a < ?b |- context [ ?a <? ?b ] ] =>
-    let X := fresh in
-    assert (a <? b = true) as X by (rewrite Nat.ltb_lt; apply H);
-    rewrite X; clear X
-  | [ |- context [ _ || true ] ] =>
-    rewrite orb_true_r
-  | [ |- context [ true || _ ] ] =>
-    rewrite orb_true_l
-  end.
 
 Lemma trace_find_previous {tid2 a2 tid1 a1 t}:
   sto_trace ((tid2, a2) :: (tid1, a1) :: t) ->
